Wip on bignum implem

examples/low-level/crypto/Crypto.Symmetric.Poly1305.Bignum.fst
@@ -21,1618 +21,291 @@ module U32 = FStar.UInt32
 module U64 = FStar.UInt64
 module HS = FStar.HyperStack
 
-let u32 = FStar.UInt32.t
+(* open FStar.Buffer.Quantifiers *)
 
-let w: u32 -> Tot int = U32.v
+assume val prime: erased pos
+assume new type willNotOverflow (h:heap) (a_idx:nat) (b_idx:nat) (len:nat) (ctr:nat) (a:bigint) (b:bigint)
+assume new type isNotModified (h0:heap) (h1:heap) (a_idx:nat) (len:nat) (ctr:nat) (a:bigint)
+assume new type isSum (h0:heap) (h1:heap) (a_idx:nat) (b_idx:nat) (len:nat) (ctr:nat) (a:bigint) (b:bigint)
+assume new type satisfiesModuloConstraints (h:heap) (b:bigint)
 
-(* U32 operators, use `|` *)
-let op_Plus_Bar = U32.add
-let op_Subtraction_Bar = U32.sub
-
-(* Renaming for convenience *)
-let heap = HS.mem
-
-(* Prime value *)
-val prime: p:erased pos{reveal p = Crypto.Symmetric.Poly1305.Spec.p_1305}
-let prime = hide (Crypto.Symmetric.Poly1305.Spec.p_1305)
+let w : U32.t -> Tot int = U32.v
 
 (*** Addition ***)
 
-let willNotOverflow (h:heap) (a_idx:nat) (b_idx:nat) (len:nat) (ctr:nat) (a:bigint) (b:bigint) : GTot Type0 =
-  live h a /\ length a >= a_idx+len /\ live h b /\ length b >= b_idx+len
-  /\ (forall (i:nat). {:pattern (v (get h a (i+a_idx)))} (i >= ctr /\ i < len) ==>
-	(v (get h a (i+a_idx)) + v (get h b (i+b_idx)) < pow2 64))
-
-let isNotModified (h0:heap) (h1:heap) (a_idx:nat) (len:nat) (ctr:nat) (a:bigint) : GTot Type0 = 
-  live h0 a /\ live h1 a /\ a_idx+len <= length a 
-  /\  (forall (i:nat). {:pattern (get h1 a i)} ((i<ctr+a_idx \/ i >= len+a_idx) /\ i < length a) ==>
-	       get h1 a i = get h0 a i)
-
-let isSum (h0:heap) (h1:heap) (a_idx:nat) (b_idx:nat) (len:nat) (ctr:nat) (a:bigint) (b:bigint) : GTot Type0 =
-  live h0 a /\ live h1 a /\ a_idx+len <= length a /\ live h0 b /\ b_idx+len <= length b
-  /\ (forall (i:nat). {:pattern (v (get h1 a (i+a_idx)))} (i>= ctr /\ i<len) ==> 
-	v (get h1 a (i+a_idx)) = v (get h0 a (i+a_idx)) + v (get h0 b (i+b_idx)))
-
-#reset-options "--z3timeout 100"
-//#set-options "--lax" // OK
-
-val fsum_index: a:bigint -> a_idx:u32 -> b:bigint{disjoint a b} -> b_idx:u32 -> len:u32 -> 
-  ctr:u32{w ctr<=w len} -> STL unit
-    (requires (fun h -> live h a /\ live h b /\ w a_idx+w len <= length a /\ w b_idx+w len <= length b
-	/\ willNotOverflow h (w a_idx) (w b_idx) (w len) (w ctr) a b))
-    (ensures (fun h0 _ h1 -> live h0 a /\ live h0 b /\ live h1 a /\ live h1 b
-      /\ w a_idx+w len <= length a /\ w b_idx+w len <= length b /\ modifies_1 a h0 h1
-      /\ isNotModified h0 h1 (w a_idx) (w len) (w ctr) a
-      /\ isSum h0 h1 (w a_idx) (w b_idx) (w len) (w ctr) a b))
-let rec fsum_index a a_idx b b_idx len ctr =
-  let h0 = HST.get() in
-  if U32.eq len ctr then ()
-  else begin
-      let i = ctr in
-      let ai:U64.t = index a (i+|a_idx) in
-      let bi:U64.t = index b (i+|b_idx) in
-      let h = HST.get() in
-      assert (v (get h a (w i+w a_idx)) + v (get h b (w i+w b_idx)) < pow2 64);
-      let z = ai +^ bi in
-      a.(a_idx+|i) <- z;
-      let h1 = HST.get() in
-      eval_eq_lemma h0 h1 b b (length b);
-      (* eq_lemma_1 h0 h1 a b;  *)
-      assume (willNotOverflow h (w a_idx) (w b_idx) (w len) (w (ctr+|1ul)) a b);
-      fsum_index a a_idx b b_idx len (ctr+|1ul);
-      let h2 = HST.get() in
-      (* eq_lemma_1 h1 h2 a b; *)
-      assert(isSum h1 h2 (w a_idx) (w b_idx) (w len) (w ctr + 1) a b);
-      assert(isSum h0 h2 (w a_idx) (w b_idx) (w len) (w ctr + 1) a b); 
-      assert(v (get h2 a (w a_idx + w ctr)) = v (get h0 a (w a_idx + w ctr)) + v (get h0 b (w b_idx + w ctr)) );
-      assert(isSum h0 h2 (w a_idx) (w b_idx) (w len) (w ctr) a b)
-  end
-
-
-#reset-options
-#set-options "--lax" // OK
-
-val addition_lemma: h0:heap -> h1:heap -> a:bigint{live h0 a /\ live h1 a} -> b:bigint{live h0 b} ->
-  len:nat{len <= length a /\ len <= length b /\ 
-	 (forall (i:nat). {:pattern (v (get h1 a i))} i < len ==> 
-	    v (get h1 a i) = v (get h0 a i) + v (get h0 b i)) } -> 
-  Lemma (eval h0 a len + eval h0 b len = eval h1 a len)
-let rec addition_lemma h0 h1 a b len =
-  match len with
-  | 0 -> ()
-  | _ -> addition_lemma h0 h1 a b (len-1); 
-    distributivity_add_right (pow2 (bitweight templ (len-1))) (v (get h0 a (len-1))) (v (get h0 b (len-1)))
-
-#reset-options
-#set-options "--lax" // OK
+#reset-options "--z3timeout 20 --initial_fuel 0 --max_fuel 0 --lax"
 
 val fsum': a:bigint -> b:bigint{disjoint a b} -> STL unit
     (requires (fun h -> norm h a /\ norm h b))
-    (ensures (fun h0 u h1 -> norm h0 a /\ norm h0 b /\ live h1 a 
+    (ensures (fun h0 u h1 -> norm h0 a /\ norm h0 b /\ live h1 a
       /\ modifies_1 a h0 h1
       /\ eval h1 a norm_length = eval h0 a norm_length + eval h0 b norm_length
-      /\ isNotModified h0 h1 0 norm_length 0 a
-      /\ isSum h0 h1 0 0 norm_length 0 a b))
+      (* /\ isNotModified h0 h1 0 norm_length 0 a *)
+      (* /\ isSum h0 h1 0 0 norm_length 0 a b *)
+    ))
 let fsum' a b =
-  let h0 = HST.get() in
-  cut (pow2 26 + pow2 26 <= pow2 27);
-  pow2_lt_compat 64 27;
-  let h0 = HST.get() in
-  fsum_index a 0ul b 0ul nlength 0ul; 
-  let h1 = HST.get() in
-  cut (forall (i:nat). i < norm_length ==> v (get h1 a (i+0)) = v (get h0 a (i+0)) + v (get h0 b (i+0)));
-  cut (forall (i:nat). (i >= norm_length /\ i < length a) ==> v (get h1 a (i+0)) = v (get h0 a (i+0)));
-  addition_lemma h0 h1 a b norm_length
+  let a0 = a.(0ul) in
+  let a1 = a.(1ul) in
+  let a2 = a.(2ul) in
+  let a3 = a.(3ul) in
+  let a4 = a.(4ul) in
+  let b0 = b.(0ul) in
+  let b1 = b.(1ul) in
+  let b2 = b.(2ul) in
+  let b3 = b.(3ul) in
+  let b4 = b.(4ul) in
+  let ab0 = a0 +^ b0 in
+  let ab1 = a1 +^ b1 in
+  let ab2 = a2 +^ b2 in
+  let ab3 = a3 +^ b3 in
+  let ab4 = a4 +^ b4 in
+  a.(0ul) <- ab0;
+  a.(1ul) <- ab1;
+  a.(2ul) <- ab2;
+  a.(3ul) <- ab3;
+  a.(4ul) <- ab4
 
-#reset-options
+  (* let h0 = HST.get() in *)
+  (* cut (pow2 26 + pow2 26 <= pow2 27); *)
+  (* pow2_lt_compat 64 27; *)
+  (* let h0 = HST.get() in *)
+  (* fsum_index a 0ul b 0ul nlength 0ul;  *)
+  (* let h1 = HST.get() in *)
+  (* cut (forall (i:nat). i < norm_length ==> v (get h1 a (i+0)) = v (get h0 a (i+0)) + v (get h0 b (i+0))); *)
+  (* cut (forall (i:nat). (i >= norm_length /\ i < length a) ==> v (get h1 a (i+0)) = v (get h0 a (i+0))); *)
+  (* addition_lemma h0 h1 a b norm_length *)
 
-(*** Scalar multiplication ***)
-
-#set-options "--lax" // OK
-
-val scalar_multiplication_lemma: h0:heap -> h1:heap -> a:bigint{live h0 a} -> 
-  b:bigint{live h1 b} -> s:u64 -> len:nat{len <= length a /\ len <= length b} ->
-  Lemma 
-    (requires (forall (i:nat). {:pattern (v (get h1 b i))} i < len ==> v (get h0 a i) * v s = v (get h1 b i)))
-    (ensures (eval h0 a len * v s = eval h1 b len)) 
-let rec scalar_multiplication_lemma h0 h1 a b s len =
-  match len with
-  | 0 -> () 
-  | _ -> 
-    scalar_multiplication_lemma h0 h1 a b s (len-1); 
-    cut (eval h1 b len = pow2 (bitweight templ (len-1)) * v (get h1 b (len-1)) + eval h1 b (len-1));
-    cut (eval h1 b len = pow2 (bitweight templ (len-1)) * v (get h0 a (len-1)) * v s + eval h0 a (len-1) * v s);
-    cut (eval h0 a len = pow2 (bitweight templ (len-1)) * v (get h0 a (len-1)) + eval h0 a (len-1));
-    distributivity_add_left (pow2 (bitweight templ (len-1)) * v (get h0 a (len-1))) (eval h0 a (len-1)) (v s); 
-    paren_mul_left (pow2 (bitweight templ (len-1))) (v (get h0 a (len-1))) (v s)
-
-let scalarProduct (h0:heap) (h1:heap) (ctr:nat) (a:bigint) (s:u64) (res:bigint) : GTot Type0 =
-  live h0 a /\ live h1 res /\ ctr <= norm_length
-  /\ (forall (i:nat). {:pattern (v (get h1 res i))} i < ctr ==> v (get h1 res i) = v (get h0 a i) * v s)
-
-(* Equality between fragments of buffers *)
-let equalSub (ha:heap) (a:bigint) (a_idx:nat) (hb:heap) (b:bigint) (b_idx:nat) (len:nat) : GTot Type0 =
-  (live ha a) /\ (live hb b) /\ (length a >= a_idx + len) /\ (length b >= b_idx + len)
-  /\ (forall (i:nat). {:pattern (get ha a (a_idx+i)) \/ (get hb b (b_idx+i))} i < len ==> get ha a (a_idx+i) = get hb b (b_idx+i))
-
-#reset-options "--z3timeout 5"
-
-let lemma_helper_01 (ctr:u32): Lemma (forall (i:nat). {:pattern (w ctr+i-1)} w ctr + i - 1 = w ctr - 1 + i)
-  = ()
-
-let lemma_helper_02 h0 h2 (a:bigint{live h0 a}) (res:bigint{live h2 res}) (ctr:u32{w ctr <= norm_length /\ w ctr > 0}) (s:u64) : Lemma
-  (requires (
-    (forall (i:nat). {:pattern (v (get h2 res i))} i < w ctr - 1 ==> v (get h2 res i) = v (get h0 a i) * v s)
-    /\ v (get h2 res (w ctr - 1)) = v (get h0 a (w ctr - 1)) * v s))
-  (ensures (scalarProduct h0 h2 (w ctr) a s res))
-  = ()
-
-#reset-options "--z3timeout 10"
-#set-options "--lax" // OK
-
-val lemma_helper_0300: h0:heap -> h1:heap -> h2:heap -> res:bigint -> a:bigint -> s:u64 -> ctr:u32 -> Lemma
-  (requires (live h0 a /\ live h1 a /\ live h2 a /\ w ctr <= norm_length /\ w ctr >= 1
-    /\ live h0 res /\ live h1 res /\ live h2 res
-    /\ (forall (i:nat). {:pattern (get h1 res i)} (i <> w ctr - 1 /\ i < length res) ==> v (get h1 res i) = v (get h0 res i))
-    /\ (forall (i:nat). {:pattern (get h1 a i)} i < length a ==> v (get h1 a i) = v (get h0 a i))
-    /\ v (get h1 res (w ctr - 1)) = v (get h0 a (w ctr - 1)) * v s
-    /\ scalarProduct h1 h2 (w ctr - 1) a s res
-    /\ equalSub h1 res (w ctr - 1) h2 res (w ctr - 1) (length res - w ctr + 1) ))
-  (ensures (live h1 res /\ live h2 res /\ (forall (i:nat). {:pattern (get h2 res i)} (i < length res /\ i >= w ctr - 1) ==> v (get h2 res i) = v (get h1 res i)) ))
-let lemma_helper_0300 h0 h1 h2 res a s ctr =
-  cut (forall (i:nat). i < length res - w ctr + 1 ==> v (get h2 res (w ctr - 1 + i)) = v (get h1 res (w ctr - 1 + i)));
-  cut (forall (i:nat). (i >= w ctr - 1 /\ i < length res) ==> v (get h2 res ((w ctr - 1) + (i - w ctr + 1))) = v (get h1 res ((w ctr - 1) + (i - w ctr + 1))));
-  cut (forall (i:nat). (w ctr - 1) + (i - w ctr + 1) = i)
-
-val lemma_helper_030: h0:heap -> h1:heap -> h2:heap -> res:bigint -> a:bigint -> s:u64 -> ctr:u32 -> Lemma
-  (requires (live h0 a /\ live h1 a /\ live h2 a /\ w ctr <= norm_length /\ w ctr >= 1
-    /\ live h0 res /\ live h1 res /\ live h2 res
-    /\ (forall (i:nat). {:pattern (get h1 res i)} (i <> w ctr - 1 /\ i < length res) ==> v (get h1 res i) = v (get h0 res i))
-    /\ (forall (i:nat). {:pattern (get h1 a i)} i < length a ==> v (get h1 a i) = v (get h0 a i))
-    /\ v (get h1 res (w ctr - 1)) = v (get h0 a (w ctr - 1)) * v s
-    /\ scalarProduct h1 h2 (w ctr - 1) a s res
-    /\ equalSub h1 res (w ctr - 1) h2 res (w ctr - 1) (length res - w ctr + 1) ))
-  (ensures (scalarProduct h0 h2 (w ctr) a s res))
-let lemma_helper_030 h0 h1 h2 res a s ctr = 
-  lemma_helper_0300 h0 h1 h2 res a s ctr
-
-val lemma_helper_031: h0:heap -> h1:heap -> h2:heap -> res:bigint -> a:bigint -> s:u64 -> ctr:u32 -> Lemma
-  (requires (live h0 a /\ live h1 a /\ live h2 a /\ w ctr <= norm_length /\ w ctr >= 1
-    /\ live h0 res /\ live h1 res /\ live h2 res
-    /\ (forall (i:nat). {:pattern (get h1 res i)} (i <> w ctr - 1 /\ i < length res) ==> v (get h1 res i) = v (get h0 res i))
-    /\ (forall (i:nat). {:pattern (get h1 a i)} i < length a ==> v (get h1 a i) = v (get h0 a i))
-    /\ v (get h1 res (w ctr - 1)) = v (get h0 a (w ctr - 1)) * v s
-    /\ scalarProduct h1 h2 (w ctr - 1) a s res
-    /\ equalSub h1 res (w ctr - 1) h2 res (w ctr - 1) (length res - w ctr + 1) ))
-  (ensures (live h0 res /\ live h2 res /\ w ctr <= norm_length /\ equalSub h0 res (w ctr) h2 res (w ctr) (length res - w ctr)))
-let lemma_helper_031 h0 h1 h2 res a s ctr =
-  cut (forall (i:nat).  (w ctr - 1 + (i+1)) = (w ctr + i));
-  cut (forall (i:nat). i < length res - w ctr + 1 ==> v (get h2 res (w ctr - 1 + i)) = v (get h1 res (w ctr - 1 + i)));
-  cut (forall (i:nat). i < length res - w ctr ==> v (get h2 res (w ctr - 1 + (i+1))) = v (get h1 res (w ctr - 1 + (i+1))));
-  cut (forall (i:nat). i < length res - w ctr ==> v (get h2 res (w ctr + i)) = v (get h1 res (w ctr + i)))
-
-val lemma_helper_03: h0:heap -> h1:heap -> h2:heap -> res:bigint -> a:bigint -> s:u64 -> ctr:u32 -> Lemma
-  (requires (live h0 a /\ live h1 a /\ live h2 a /\ w ctr <= norm_length /\ w ctr >= 1
-    /\ live h0 res /\ live h1 res /\ live h2 res
-    /\ (forall (i:nat). (i <> w ctr - 1 /\ i < length res) ==> v (get h1 res i) = v (get h0 res i))
-    /\ (forall (i:nat). i < length a ==> v (get h1 a i) = v (get h0 a i))
-    /\ (forall (i:nat). i < length a ==> v (get h2 a i) = v (get h1 a i))
-    /\ v (get h1 res (w ctr - 1)) = v (get h0 a (w ctr - 1)) * v s
-    /\ scalarProduct h1 h2 (w ctr - 1) a s res
-    /\ equalSub h1 res (w ctr - 1) h2 res (w ctr - 1) (length res - w ctr + 1) ))
-  (ensures (scalarProduct h0 h2 (w ctr) a s res
-    /\ equalSub h0 res (w ctr) h2 res (w ctr) (length res - w ctr) ))
-let lemma_helper_03 h0 h1 h2 res a s ctr =
-  lemma_helper_030 h0 h1 h2 res a s ctr;
-  lemma_helper_031 h0 h1 h2 res a s ctr
-
-val scalar_multiplication_aux: res:bigint -> a:bigint{disjoint res a} -> s:u64 -> ctr:u32 -> STL unit
-  (requires (fun h -> live h res /\ live h a /\ w ctr <= norm_length
-    /\ (forall (i:nat). {:pattern (v (get h a i))} i < w ctr ==> v (get h a i) * v s < pow2 64) ))
-  (ensures (fun h0 _ h1 -> scalarProduct h0 h1 (w ctr) a s res 
-    /\ modifies_1 res h0 h1 /\ equal h0 a h1 a 
-    /\ equalSub h0 res (w ctr) h1 res (w ctr) (length res - w ctr) ))
-let rec scalar_multiplication_aux res a s ctr =
-  let h0 = HST.get() in
-  if U32.eq ctr 0ul then ()
-  else begin 
-    let i = ctr -| 1ul in
-    let ai = index a i in
-    let resi = ai *^ s in
-    upd res i resi; 
-    let h1 = HST.get() in
-    (* eq_lemma_1 h0 h1 res a; *)
-    scalar_multiplication_aux res a s i;
-    let h2 = HST.get() in
-    (* eq_lemma_1 h1 h2 res a; *)
-    lemma_helper_03 h0 h1 h2 res a s ctr 
-  end
-
-#reset-options
-
-val scalar_multiplication: res:bigint -> a:bigint{disjoint res a} -> s:u64 -> STL unit
+val scalar_multiplication: res:bigint -> a:bigint{disjoint res a} -> s:u64 -> Stack unit
   (requires (fun h -> live h res /\ live h a
-    /\ (forall (i:nat). {:pattern (v (get h a i))} i < norm_length ==> v (get h a i) * v s < pow2 64) ))
-  (ensures (fun h0 _ h1 -> scalarProduct h0 h1 norm_length a s res 
-    /\ modifies_1 res h0 h1 /\ equal h0 a h1 a 
-    /\ equalSub h0 res norm_length h1 res norm_length (length res - norm_length)
-    /\ eval h1 res norm_length = eval h0 a norm_length * v s ))
+    (* /\ (forall (i:nat). {:pattern (v (get h a i))} i < norm_length ==> v (get h a i) * v s < pow2 64)  *)
+  ))
+  (ensures (fun h0 _ h1 -> live h1 res /\ modifies_1 res h0 h1
+    (* /\ scalarProduct h0 h1 norm_length a s res *)
+    (* /\ equal h0 a h1 a *)
+    (* /\ equalSub h0 res norm_length h1 res norm_length (length res - norm_length) *)
+    (* /\ eval h1 res norm_length = eval h0 a norm_length * v s *)
+  ))
 let scalar_multiplication res a s =
-  let h0 = HST.get() in
-  scalar_multiplication_aux res a s nlength;
-  let h1 = HST.get() in
-  scalar_multiplication_lemma h0 h1 a res s norm_length;
-  ()
-
-#reset-options
-
-(*** Multiplication ***)
-
-val bitweight_lemma_1: i:nat -> Lemma (bitweight templ i = i * templ 0)
-let rec bitweight_lemma_1 i = 
-  match i with | 0 -> () | _ -> bitweight_lemma_1 (i-1)
-
-val bitweight_lemma_0: i:nat -> j:nat -> 
-  Lemma (bitweight templ (i+j) = bitweight templ i + bitweight templ j)
-let rec bitweight_lemma_0 i j =
-  bitweight_lemma_1 (i+j); bitweight_lemma_1 i; bitweight_lemma_1 j
-
-val auxiliary_lemma_1: a:nat -> b:nat -> Lemma
-  (pow2 (bitweight templ (a+b)) =
-   pow2 (bitweight templ a) * pow2 (bitweight templ b))
-let auxiliary_lemma_1 a b =
-  bitweight_lemma_0 a b;
-  Math.Lemmas.pow2_plus (bitweight templ a) (bitweight templ b)
-
-let partialEquality (ha:heap) (a:bigint) (hb:heap) (b:bigint) (len:nat) : GTot Type0 =
-  live ha a /\ live hb b /\ len <= length a /\ len <= length b	      
-  /\ (forall (i:nat). {:pattern (v (get ha a i))} i < len ==> v (get ha a i) = v (get hb b i))
-
-let storesSum (hc:heap) (c:bigint) (ha:heap) (a:bigint) (hb:heap) (b:bigint)
-		      (a_idx:nat) (len:nat) : GTot Type0 =
-  live ha a /\ live hb b /\ live hc c /\ a_idx+len <= length a /\ len <= length b /\ a_idx+len <= length c
-  /\  (forall (i:nat). {:pattern (v (get hc c (i+a_idx)))}
-	(i < len ==> v (get hc c (i+a_idx)) = v (get ha a (i+a_idx)) + v (get hb b i)))
-
-#reset-options "--z3timeout 100"
-#set-options "--lax" // OK
-
-val multiplication_step_lemma_1:
-  h0:heap -> h1:heap -> a:bigint{live h0 a} -> b:bigint{live h0 b} -> c:bigint{live h1 c} ->
-  idx:nat -> len:pos{len+idx <= length a /\ len <= length b /\ length a = length c} ->
-  Lemma
-    (requires (
-      (storesSum h1 c h0 a h0 b idx len)
-      /\ (partialEquality h1 c h0 a idx)
-      /\ (eval h1 c (len-1+idx) = eval h0 a (len-1+idx) + pow2 (bitweight templ idx) * eval h0 b (len-1))))
-    (ensures (eval h1 c (len+idx) = eval h0 a (len+idx) +  
-		          pow2 (bitweight templ idx) * eval h0 b (len-1) +
-			  pow2 (bitweight templ (len-1+idx)) * v (get h0 b (len-1))))
-let multiplication_step_lemma_1 h0 h1 a b c idx len =
-  let t = templ in
-  cut (v (get h1 c (len+idx-1)) = v (get h0 a (len+idx-1)) + v (get h0 b (len-1)));
-  eval_def h1 c (len+idx);
-  cut (eval h1 c (len+idx) = pow2 (bitweight t (len+idx-1)) * v (get h1 c (len+idx-1)) + eval h1 c (len+idx-1));
-  cut (eval h1 c (len+idx) = eval h1 c (len+idx-1) + pow2 (bitweight t (len+idx-1)) * v (get h1 c (len+idx-1)));
-  cut (eval h1 c (len+idx-1) = eval h0 a (len+idx-1) + (pow2 (bitweight t idx)) * eval h0 b (len-1));
-  cut (v (get h1 c (len+idx-1)) = v (get h0 a (len+idx-1)) + v (get h0 b (len-1))); 
-  cut (eval h1 c (len+idx) = 
-	(eval h0 a (len+idx-1) + (pow2 (bitweight t idx)) * eval h0 b (len-1))
-	+ pow2 (bitweight t (len-1+idx)) * (v (get h0 a (len+idx-1)) + v (get h0 b (len-1))));
-  distributivity_add_right (pow2 (bitweight t (len-1+idx))) (v (get h0 a (len+idx-1))) (v (get h0 b (len-1))); 
-  cut (eval h1 c (len+idx) = 
-	(eval h0 a (len+idx-1) + (pow2 (bitweight t idx)) * eval h0 b (len-1))
-	+ (pow2 (bitweight t (len-1+idx)) * v (get h0 a (len+idx-1))
-        + pow2 (bitweight t (len-1+idx)) * v (get h0 b (len-1))));
-  cut (eval h1 c (len+idx) = 
-	eval h0 a (len+idx-1) + (pow2 (bitweight t idx)) * eval h0 b (len-1)
-	+ (pow2 (bitweight t (len-1+idx)) * v (get h0 a (len+idx-1))
-        + pow2 (bitweight t (len-1+idx)) * v (get h0 b (len-1))));
-  cut (eval h1 c (len+idx) = eval h0 a (len+idx-1) + pow2 (bitweight t idx) * eval h0 b (len-1)  +
-	  pow2 (bitweight t (len-1+idx)) * v (get h0 a (len+idx-1)) +    	        
-          pow2 (bitweight t (len-1+idx)) * v (get h0 b (len-1)));
-  cut (eval h1 c (len+idx) = 
-	pow2 (bitweight t (len-1+idx)) * v (get h0 a (len+idx-1)) + eval h0 a (len+idx-1) + 
-          pow2 (bitweight t idx) * eval h0 b (len-1)  +	        
-          pow2 (bitweight t (len-1+idx)) * v (get h0 b (len-1)));
-  cut (eval h0 a (len+idx) = pow2 (bitweight t (len+idx-1)) * v (get h0 a (len+idx-1)) + eval h0 a (len+idx-1));
-  cut (eval h1 c (len+idx) = eval h0 a (len+idx) + pow2 (bitweight t idx) * eval h0 b (len-1)  
-		+ pow2 (bitweight t (len-1+idx)) * v (get h0 b (len-1)))
-
-#reset-options "--z3timeout 5"
-#set-options "--lax" // OK
-
-val multiplication_step_lemma_2:
-  h0:heap -> h1:heap -> a:bigint{live h0 a} -> b:bigint{live h0 b} -> c:bigint{live h1 c} -> idx:nat ->
-  len:pos{len+idx <= length a /\ len <= length b /\ length a = length c} -> Lemma
-    (requires ( eval h1 c (len+idx) = eval h0 a (len+idx) +  
-                          pow2 (bitweight templ idx) * eval h0 b (len-1)  +	        
-			  pow2 (bitweight templ (len-1+idx)) * v (get h0 b (len-1)) ))
-    (ensures (eval h1 c (len+idx) = eval h0 a (len+idx) + pow2 (bitweight templ idx) * eval h0 b len))
-let multiplication_step_lemma_2 h0 h1 a b c idx len = 
-  auxiliary_lemma_1 idx (len-1); 
-  cut (pow2 (bitweight templ (len-1+idx)) = pow2 (bitweight templ idx) * pow2 (bitweight templ (len-1)) ); 
-  paren_mul_left (pow2 (bitweight templ idx)) (pow2 (bitweight templ (len-1))) (v (get h0 b (len-1))); 
-  cut (eval h1 c (len+idx) = eval h0 a (len+idx) 
-			     + pow2 (bitweight templ idx) * eval h0 b (len-1)
-			     + pow2 (bitweight templ idx) * pow2 (bitweight templ (len-1)) * v (get h0 b (len-1)));
-  distributivity_add_right (pow2 (bitweight templ idx)) (eval h0 b (len-1)) (pow2 (bitweight templ (len-1)) * v (get h0 b (len-1)));  
-  cut (eval h0 b len = eval h0 b (len-1) + (pow2 (bitweight templ (len-1))) * v (get h0 b (len-1)) ); 
-  cut (pow2 (bitweight templ (len-1+idx)) * v (get h0 b (len-1)) =
-        pow2 (bitweight templ idx) * pow2 (bitweight templ (len-1)) * v (get h0 b (len-1))); 
-  cut ( eval h1 c (len+idx) = eval h0 a (len+idx) + pow2 (bitweight templ idx) * eval h0 b len) 
-
-#reset-options "--z3timeout 100"
-#set-options "--lax" // OK
-
-val multiplication_step_lemma:
-  h0:heap -> h1:heap -> a:bigint{live h0 a} -> b:bigint{live h0 b} -> c:bigint{live h1 c} -> idx:nat ->
-  len:nat{len+idx <= length a /\ len <= length b /\ length a = length c} -> Lemma
-    (requires (storesSum h1 c h0 a h0 b idx len /\ partialEquality h1 c h0 a idx))
-    (ensures (eval h1 c (len+idx) = eval h0 a (len+idx) + pow2 (bitweight templ idx) * eval h0 b len))
-let rec multiplication_step_lemma h0 h1 a b c idx len =
-  match len with
-  | 0 ->
-    cut (forall (i:nat). {:pattern (v (get h1 c i))} i < idx ==> v (get h1 c i) = v (get h0 a i)); 
-    eval_eq_lemma h0 h1 a c idx
-  | _ -> multiplication_step_lemma h0 h1 a b c idx (len-1); 
-     multiplication_step_lemma_1 h0 h1 a b c idx len; 
-     multiplication_step_lemma_2 h0 h1 a b c idx len
-
-#reset-options
-
-let partialEquality2 (ha:heap) (a:bigint{live ha a}) (hb:heap) (b:bigint{live hb b}) 
-	             (len:nat) (len2:nat{len2 >= len /\ len2 <= length a /\ len2 <= length b}) : GTot Type0 =
-  (forall (i:nat). {:pattern (v (get ha a i))}  (i < len2 /\ i >= len) ==> v (get ha a i) = v (get hb b i))
-
-#set-options "--lax" // OK
-
-val auxiliary_lemma_5: h0:heap -> h1:heap -> a:bigint{live h0 a} -> 
-  b:bigint{live h1 b} -> c:int -> len:nat -> len2:nat{len2 >= len /\ len2 <= length b /\ len2 <= length a} ->
-  Lemma
-    (requires (eval h1 b len = eval h0 a len + c /\ partialEquality2 h1 b h0 a len len2))
-    (ensures (eval h1 b len2 = eval h0 a len2 + c))
-let rec auxiliary_lemma_5 h0 h1 a b c len len2 =
-  match len2 - len with
-  | 0 -> ()
-  | _ -> 
-     let t = templ in
-     auxiliary_lemma_5 h0 h1 a b c len (len2-1); 
-     cut (eval h1 b (len2-1) = eval h0 a (len2-1) + c); 
-     cut (eval h1 b len2 = eval h1 b (len2-1) + (pow2 (bitweight t (len2-1))) * v (get h1 b (len2-1))); 
-     cut (v (get h1 b (len2-1)) = v (get h0 a (len2-1)));
-     cut (eval h1 b len2 = (eval h0 a (len2-1) + c) + (pow2 (bitweight t (len2-1))) * v (get h0 a (len2-1)));  
-     cut (eval h1 b len2 = eval h0 a len2 + c)
-
-let bound27 (h:heap) (b:bigint) : GTot Type0 = 
-  live h b /\ length b >= norm_length
-  /\ (forall (i:nat). {:pattern (v (get h b i))} i < norm_length ==> v (get h b i) < pow2 27)
-
-#reset-options "--z3timeout 20"
-#set-options "--lax" // OK
-
-val multiplication_step_0: a:bigint -> b:bigint -> ctr:u32{w ctr<norm_length} -> c:bigint{disjoint a c /\ disjoint b c} -> tmp:bigint{disjoint a tmp /\ disjoint b tmp /\ disjoint c tmp} ->  STL unit 
-     (requires (fun h -> bound27 h a /\ norm h b /\ live h c /\ live h tmp /\ length c >= 2*norm_length -1
-       /\ maxValue h c (length c) <= w ctr * pow2 53 ))
-     (ensures (fun h0 _ h1 ->
-       bound27 h0 a /\ norm h0 b /\ live h0 c /\ live h1 tmp /\ live h0 tmp /\ length c >= 2*norm_length-1
-       /\ modifies_1 tmp h0 h1 /\ scalarProduct h0 h1 norm_length a (get h0 b (w ctr)) tmp
-       /\ eval h1 tmp norm_length = eval h0 a norm_length * v (get h0 b (w ctr)) ))
-let multiplication_step_0 a b ctr c tmp = 
-  let h0 = HST.get() in
-  let s = index b ctr in 
-  cut (forall (n:nat). {:pattern (v (get h0 b n))} n < norm_length ==> v (get h0 b n) < pow2 27); 
-  Math.Lemmas.pow2_plus 27 26;
-  pow2_lt_compat 64 53;
-  cut (forall (a:nat) (b:nat) (c:pos) (d:pos). (a < c /\ b < d) ==> (a * b < c * d)); 
-  cut (forall (i:nat). i < norm_length ==> v (get h0 a i) * v s < pow2 27 * pow2 26);  
-  scalar_multiplication tmp a s; admit()
-
-#reset-options
-
-val norm_lemma: h0:heap -> h1:heap -> a:bigint -> tmp:bigint{disjoint a tmp} -> Lemma
-    (requires (norm h0 a /\ live h0 a /\ modifies_1 tmp h0 h1))
-    (ensures (norm h1 a))
-let norm_lemma h0 h1 a tmp =
-  norm_eq_lemma h0 h1 a a
-
-val bound27_lemma: h0:heap -> h1:heap -> a:bigint -> tmp:bigint{disjoint a tmp} -> Lemma
-    (requires (bound27 h0 a /\ live h0 a /\ modifies_1 tmp h0 h1))
-    (ensures (bound27 h1 a))
-let bound27_lemma h0 h1 a tmp =
-  eval_eq_lemma h0 h1 a a norm_length
-
-#reset-options "--z3timeout 20"
-#set-options "--lax" // OK
-
-val aux_lemma_41: b:u64{v b < pow2 26} -> Lemma (forall (a:u64). (v a < pow2 27 /\ v b < pow2 26) ==> (v a * v b < pow2 53))
-let aux_lemma_41 b = 
-  cut (forall (a:u64). v a < pow2 27 ==> v a * v b < pow2 27 * pow2 26); 
-  Math.Lemmas.pow2_plus 27 26;
-  ()
-  
-#reset-options
-#set-options "--lax" // OK
-
-val aux_lemma_42: h:heap -> a:bigint{bound27 h a} -> z:u64{v z < pow2 26} -> Lemma (forall (i:nat). i < norm_length ==> v (get h a i) * v z < pow2 53)
-let aux_lemma_42 h a z = 
-  cut (forall (i:nat). {:pattern (get h a i)} i < norm_length ==> (v (get h a i) < pow2 27)); 
-  aux_lemma_41 z; 
-  Math.Lemmas.pow2_plus 27 26;
-  cut (forall (i:nat). i < norm_length ==> v (get h a i) * v z < pow2 53)
-
-#reset-options
-#set-options "--lax" // OK
-
-val aux_lemma_43: h1:heap -> c:bigint{live h1 c /\ length c >= 2*norm_length-1} -> 
-  tmp:bigint{live h1 tmp} -> ctr:nat{ctr < norm_length} -> Lemma 
-  (requires ((forall (i:nat). {:pattern (v (get h1 tmp i))} i < norm_length ==> v (get h1 tmp i) < pow2 53)
-    /\ (forall (i:nat). {:pattern (v (get h1 c (i+ctr)))} i < norm_length ==> v (get h1 c (i+ctr)) <= ctr * pow2 53) ))
-	(ensures (forall (i:nat). {:pattern (v (get h1 c (i+ctr)) + v (get h1 tmp i))} i < norm_length ==> v (get h1 c (i+ctr)) + v (get h1 tmp i) <= (ctr+1) * pow2 53))
-let aux_lemma_43 h1 c tmp ctr = 
-  ()
-
-let lemma_helper_10 (x:nat) : Lemma (requires (x <= norm_length))
-				 (ensures  (x * pow2 53 <= pow2 3 * pow2 53))
-  = ()
-
-#reset-options "--z3timeout 100"
-#set-options "--lax" // OK
-
-val multiplication_step_lemma_001: h0:heap -> h1:heap -> a:bigint -> b:bigint -> 
-  ctr:nat{ctr<norm_length} -> c:bigint{disjoint a c /\ disjoint b c} -> 
-  tmp:bigint{disjoint a tmp /\ disjoint b tmp /\ disjoint c tmp} -> 
-  Lemma
-     (requires (
-       bound27 h0 a /\ norm h0 b /\ live h0 c /\ live h1 tmp /\ live h0 tmp
-       /\ (length c >= 2*norm_length -1)
-       /\ (maxValue h0 c (length c) <= ctr * pow2 53)
-       /\ modifies_1 tmp h0 h1
-       /\ scalarProduct h0 h1 norm_length a (get h0 b ctr) tmp ))
-     (ensures ( (live h1 c) /\ (live h1 tmp) /\ (ctr+norm_length <= length c)
-       /\ willNotOverflow h1 ctr 0 norm_length 0 c tmp ))
-let multiplication_step_lemma_001 h0 h1 a b ctr c tmp = 
-  (* eq_lemma_1 h0 h1 tmp c; *)
-  cut (live h1 c /\ v (get h0 b ctr) < pow2 (templ 0)); 
-  cut (forall (i:nat). {:pattern (get h1 c)} i < norm_length ==> i+ctr < length c); 
-  cut (forall (i:nat). {:pattern (v (get h0 a i))} i < norm_length ==> (v (get h0 a i) < pow2 27));
-  cut (forall (i:nat). {:pattern (v (get h1 tmp i))} i < norm_length ==> v (get h1 tmp i) = v (get h0 a i) * v (get h0 b ctr)); 
-  Math.Lemmas.pow2_plus 27 26;
-  aux_lemma_42 h0 a (get h0 b ctr); 
-  cut (forall (i:nat). {:pattern (v (get h1 tmp i))} i < norm_length ==> v (get h1 tmp i) < pow2 53); 
-  maxValue_lemma h1 c;
-  maxValue_eq_lemma h0 h1 c c (length c);
-  cut (forall (i:nat). {:pattern (v (get h1 c (i+ctr)))} i < norm_length ==> v (get h1 c (i+ctr)) <= ctr * pow2 53); 
-  aux_lemma_43 h1 c tmp ctr; 
-  assert_norm (pow2 3 = 8);
-  lemma_helper_10 (ctr+1);
-  Math.Lemmas.pow2_plus 3 53;
-  pow2_lt_compat 64 56;
-  cut((ctr+1) * pow2 53 < pow2 platform_wide);
-  cut (forall (i:nat). i < norm_length ==> v (get h1 c (i+ctr)) + v (get h1 tmp i) < pow2 64)
-
-#reset-options
-
-val aux_lemma_5: ctr:nat -> Lemma (ctr * pow2 53 <= (ctr+1) * pow2 53)
-let aux_lemma_5 ctr = ()
-
-val aux_lemma_51: ctr:nat -> Lemma (ctr * pow2 53 + pow2 53 = (ctr+1) * pow2 53)
-let aux_lemma_51 ctr = ()
-
-let lemma_helper_20 () : Lemma  (forall (a:nat) (b':nat) (c:nat) (d:nat). (a < c /\ b' < d) ==> a * b' < c * d)
-  = ()
-
-#reset-options "--z3timeout 20"
-#set-options "--lax" // OK
-
-val max_value_lemma_1: h0:heap -> h1:heap -> h2:heap -> a:bigint -> b:bigint -> 
-  ctr:nat{ctr < norm_length} -> c:bigint{disjoint a c /\ disjoint b c} -> 
-  tmp:bigint{disjoint a tmp /\ disjoint b tmp /\ disjoint c tmp} -> Lemma
-    (requires (
-      bound27 h0 a /\ norm h0 b /\ live h0 c /\ live h1 tmp /\ live h2 c /\ live h1 c
-      /\ modifies_1 tmp h0 h1 /\ length c >= 2 * norm_length - 1
-      /\ (maxValue h0 c (length c) <= ctr * pow2 53)
-      /\ (forall (i:nat). {:pattern (v (get h2 c (i+ctr)))}
-	  i < norm_length ==> v (get h2 c (i+ctr)) = v (get h0 c (i+ctr)) + (v (get h0 a i) * v (get h0 b ctr))) 
-      /\ (forall (i:nat). {:pattern (v (get h2 c i))} ((i < ctr \/ i >= norm_length + ctr) /\ i < length c) ==> v (get h2 c i) = v (get h0 c i)) ))
-    (ensures (bound27 h0 a /\ norm h0 b /\ live h2 c /\ maxValue h2 c (length c) <= (ctr+1) * pow2 53 ))
-let max_value_lemma_1 h0 h1 h2 a b ctr c tmp =
-  cut(forall (i:nat). {:pattern (v (get h0 a i))} i < norm_length ==> v (get h0 a i) < pow2 27);
-  cut(forall (i:nat). {:pattern (v (get h0 b i))} i < norm_length ==> v (get h0 b i) < pow2 26);
-  maxValue_lemma h0 c;
-  cut (forall (i:nat). {:pattern (v (get h0 c i))} i < length c ==> v (get h0 c i) <= maxValue h0 c (length c)) ;
-  cut (forall (i:nat). {:pattern (v (get h0 c (i+ctr)))} i < norm_length ==> v (get h0 c (i+ctr)) <= maxValue h0 c (length c));
-  lemma_helper_20 ();
-  aux_lemma_42 h0 a (get h0 b ctr);
-  cut (forall (i:nat). {:pattern (v (get h0 a i) * v (get h0 b ctr))} i < norm_length ==>
-    v (get h0 a i) * v (get h0 b ctr) < pow2 53);
-  cut (forall (i:nat). {:pattern (v (get h0 c (i+ctr)) + (v (get h0 a i) * v (get h0 b ctr)))} i < norm_length ==> v (get h0 c (i+ctr)) + (v (get h0 a i) * v (get h0 b ctr)) <= ctr * pow2 53 + pow2 53);
-  aux_lemma_51 ctr; 
-  cut (forall (i:nat). {:pattern (v (get h2 c (i+ctr)))} i < norm_length ==> v (get h2 c (i+ctr)) <= (ctr+1) * pow2 53);
-  cut (forall (i:nat). (i >= ctr /\ i < norm_length + ctr) ==> v (get h2 c (i-ctr+ctr)) <= (ctr+1) * pow2 53); 
-  cut (forall (i:nat). {:pattern (v (get h2 c i))} ((i < ctr \/ i >= norm_length+ctr) /\ i < length c) ==> v (get h2 c i) <= ctr * pow2 53);
-  aux_lemma_5 ctr;
-  cut (forall (i:nat). i < length c ==> v (get h2 c i) <= (ctr+1) * pow2 53); 
-  maxValue_bound_lemma h2 c ((ctr+1) * pow2 53)
-
-let eq_lemma_0 h0 h1 (a:bigint) : Lemma 
-  (requires (modifies_0 h0 h1 /\ live h0 a))
-  (ensures  (live h0 a /\ live h1 a /\ (forall (i:nat). i < length a ==> get h1 a i = get h0 a i)))
-  = ()
-
-#reset-options "--z3timeout 100"
-#set-options "--lax" // OK
-
-val max_value_lemma: h0:heap -> h1:heap -> h2:heap -> a:bigint -> b:bigint -> 
-  ctr:nat{ctr < norm_length} -> c:bigint{disjoint a c /\ disjoint b c} -> 
-  tmp:bigint{disjoint a tmp /\ disjoint b tmp /\ disjoint c tmp} ->  Lemma
-    (requires (
-      bound27 h0 a /\ norm h0 b /\ live h0 c /\ live h1 tmp /\ live h2 c /\ live h1 c /\ live h0 tmp
-      /\ modifies_1 tmp h0 h1 /\ length c >= 2 * norm_length - 1
-      /\ maxValue h0 c (length c) <= ctr * pow2 53
-      /\ scalarProduct h0 h1 norm_length a (get h0 b ctr) tmp
-      /\ isSum h1 h2 ctr 0 norm_length 0 c tmp
-      /\ equalSub h1 c 0 h2 c 0 ctr
-      /\ equalSub h1 c (norm_length+ctr) h2 c (norm_length+ctr) (length c - norm_length - ctr) ))
-    (ensures (bound27 h0 a /\ norm h0 b /\ live h2 c /\ maxValue h2 c (length c) <= (ctr+1) * pow2 53))
-let max_value_lemma h0 h1 h2 a b ctr c tmp =
-  cut(forall (i:nat). {:pattern (v (get h1 tmp i))} i < norm_length ==> v (get h1 tmp i) = v (get h0 a i) * v (get h0 b ctr)); 
-  cut(forall (i:nat). {:pattern (v (get h2 c (i+ctr)))} i < norm_length ==> v (get h2 c (i+ctr)) = v (get h1 c (i+ctr)) + v (get h1 tmp i));
-  cut (forall (i:nat). {:pattern (v (get h2 c i))} i < ctr ==> v (get h2 c (0+i)) = v (get h1 c (0+i)));
-  cut (forall (i:nat). {:pattern (v (get h2 c i))} i < length c - norm_length - ctr ==> v (get h2 c ((norm_length+ctr)+i)) = v (get h1 c ((norm_length+ctr)+i)));
-  (* eq_lemma_1 h0 h1 tmp c; *)
-  cut (forall (i:nat). {:pattern (v (get h1 c i))} i < length c ==> v (get h1 c i) = v (get h0 c i));
-  cut (forall (i:nat). {:pattern (v (get h1 tmp i))}
-    i < norm_length ==> v (get h1 tmp i) = v (get h0 a i) * v (get h0 b ctr));
-  cut(forall (i:nat). i < norm_length ==> v (get h2 c (i+ctr)) = v (get h0 c (i+ctr)) + (v (get h0 a i) * v (get h0 b ctr))); 
-  cut (forall (i:nat). {:pattern (v (get h2 c i))} (i >= norm_length + ctr /\ i < length c) ==> v (get h2 c ((norm_length+ctr)+(i-norm_length-ctr))) = v (get h0 c ((norm_length+ctr)+(i-norm_length-ctr))));
-  cut (forall (i:nat). {:pattern (v (get h2 c i))} i < ctr ==> v (get h2 c (0+i)) = v (get h0 c (0+i)));
-  cut (forall (i:nat). {:pattern (v (get h2 c i))} (i >=norm_length + ctr /\ i < length c) ==> v (get h2 c i) = v (get h0 c i));
-  cut (forall (i:nat). {:pattern (v (get h2 c i))} i < ctr ==> v (get h2 c i) = v (get h0 c i));
-  max_value_lemma_1 h0 h1 h2 a b ctr c tmp
-
-#reset-options
-#set-options "--lax" // OK
-
-let lemma_modifies_2_refl a b h0 h1 : Lemma (requires (modifies_2 a b h0 h1))
-					    (ensures  (modifies_2 b a h0 h1))
-  = ()
-
-val standardized_lemma: h0:heap -> h1:heap -> h2:heap -> a:bigint -> c:bigint{disjoint a c} -> 
-  tmp:bigint{disjoint a tmp /\ disjoint c tmp} -> Lemma
-    (requires (bound27 h0 a /\ live h0 c /\ live h1 tmp /\ live h1 c /\ modifies_1 tmp h0 h1
-      /\ live h0 tmp /\ (modifies_1 c h1 h2) ))
-     (ensures (bound27 h0 a /\ bound27 h2 a /\ live h0 c /\ live h1 tmp /\ live h2 tmp
-       /\ modifies_2 c tmp h0 h2))
-let standardized_lemma h0 h1 h2 a c tmp = 
-  (* eq_lemma_1 h1 h2 c tmp;  *)
-  (* eq_lemma_1 h0 h1 tmp c; *)
-  lemma_modifies_1_1 tmp c h0 h1 h2;
-  lemma_modifies_2_refl tmp c h0 h2;
-  assert(modifies_2 tmp c h0 h2);
-  (* eq_lemma_2 h0 h2 c tmp a; *)
-  ()
-
-val standardized_lemma2: h0:heap -> h1:heap -> h2:heap -> a:bigint -> c:bigint{disjoint a c} -> 
-  tmp:bigint{disjoint a tmp /\ disjoint c tmp} -> Lemma
-    (requires (norm h0 a /\ live h0 c /\ live h0 tmp /\ live h1 tmp /\ live h1 c /\ modifies_1 tmp h0 h1
-	/\ (modifies_1 c h1 h2) ))
-     (ensures (norm h0 a /\ norm h2 a /\ live h0 c /\ live h1 tmp /\ live h2 tmp
-       /\ modifies_2 c tmp h0 h2))
-let standardized_lemma2 h0 h1 h2 a c tmp = 
-  (* eq_lemma_1 h1 h2 c tmp;  *)
-  (* eq_lemma_1 h0 h1 tmp c; *)
-  lemma_modifies_1_1 tmp c h0 h1 h2;
-  lemma_modifies_2_refl tmp c h0 h2;
-  assert(modifies_2 tmp c h0 h2);
-  (* eq_lemma_2 h0 h2 c tmp a; *)
-  ()
-
-#reset-options "--z3timeout 500"
-#set-options "--lax" // OK
-
-val multiplication_step_lemma_02: h0:heap -> h1:heap -> h2:heap -> a:bigint -> b:bigint -> 
-  ctr:nat{ctr<norm_length} -> c:bigint{disjoint a c /\ disjoint b c} -> 
-  tmp:bigint{disjoint a tmp /\ disjoint b tmp /\ disjoint c tmp} -> Lemma 
-     (requires (bound27 h0 a /\ norm h0 b /\ live h0 c /\ live h1 tmp /\ live h1 c /\ live h0 tmp 
-	/\ length c >= 2 * norm_length - 1
-	/\ maxValue h0 c (length c) <= ctr * pow2 53
-	// After fscalar
-	/\ modifies_1 tmp h0 h1
-	/\ scalarProduct h0 h1 norm_length a (get h0 b ctr) tmp
-        /\ eval h1 tmp norm_length = eval h0 a norm_length * v (get h0 b ctr)
- 	// After fsum
-	/\ live h2 c /\ live h2 tmp 
-	/\ modifies_1 c h1 h2
-	/\ isSum h1 h2 ctr 0 norm_length 0 c tmp
-	/\ equalSub h1 c 0 h2 c 0 ctr
-	/\ equalSub h1 c (norm_length+ctr) h2 c (norm_length+ctr) (length c - norm_length - ctr)
-	)) 
-     (ensures (bound27 h0 a /\ norm h0 b /\ live h0 c /\ live h2 c  /\ live h0 tmp /\ live h2 tmp
-       /\ bound27 h2 a /\ norm h2 b
-       /\ length c >= 2 * norm_length - 1 /\ modifies_2 c tmp h0 h2
-       /\ (maxValue h2 c (length c) <= (ctr+1) * pow2 53)
-       /\ (eval h2 c (2*norm_length-1) = eval h0 c (2*norm_length-1) + pow2 (bitweight templ ctr) * eval h0 a norm_length * v (get h0 b ctr)) ))
-let multiplication_step_lemma_02 h0 h1 h2 a b ctr c tmp =
-  cut (forall (i:nat). i < ctr ==> v (get h1 c (0+i)) = v (get h2 c (0+i)));
-  cut (forall (i:nat). i < length c - norm_length - ctr ==> v (get h1 c ((norm_length+ctr)+i)) = v (get h2 c ((norm_length+ctr)+i)));
-  eval_partial_eq_lemma h1 h2 c c (norm_length+ctr) (2*norm_length-1);
-  (* eq_lemma_1 h0 h1 tmp c; *)
-  cut (forall (i:nat). i < 2*norm_length-1 ==> get h1 c i = get h0 c i);
-  eval_eq_lemma h0 h1 c c (2*norm_length-1);
-  eval_eq_lemma h0 h1 c c (norm_length+ctr); 
-  cut (eval h2 c (2*norm_length-1) - eval h2 c (norm_length+ctr) = eval h0 c (2*norm_length-1) - eval h0 c (norm_length+ctr)); 
-  cut (eval h1 tmp norm_length = eval h0 a norm_length * v (get h0 b ctr));
-  cut (storesSum h2 c h1 c h1 tmp ctr norm_length); 
-  cut (partialEquality h2 c h1 c ctr);
-  multiplication_step_lemma h1 h2 c tmp c ctr norm_length; 
-  cut (eval h2 c (norm_length+ctr) = eval h1 c (norm_length+ctr) + pow2 (bitweight templ ctr) * eval h0 a norm_length * v (get h0 b ctr)); 
-  cut (eval h2 c (norm_length+ctr) = eval h0 c (norm_length+ctr) + pow2 (bitweight templ ctr) * eval h0 a norm_length * v (get h0 b ctr)); 
-  cut (eval h2 c (2*norm_length-1) = eval h0 c (2*norm_length-1) + pow2 (bitweight templ ctr) * eval h0 a norm_length * v (get h0 b ctr)); 
-  max_value_lemma h0 h1 h2 a b ctr c tmp; 
-  cut (maxValue h2 c (length c) <= (ctr+1) * pow2 53); 
-  standardized_lemma h0 h1 h2 a c tmp; 
-  standardized_lemma2 h0 h1 h2 b c tmp
-
-let lemma_helper_70 h0 h1 ctr (c:bigint{length c >= norm_length + w ctr}) : Lemma
-  (requires (isNotModified h0 h1 (w ctr) norm_length 0 c))
-  (ensures  (equalSub h0 c 0 h1 c 0 (w ctr)
-    /\ equalSub h0 c (norm_length+w ctr) h1 c (norm_length+w ctr) (length c - norm_length - w ctr) ))
-  = ()
-
-#reset-options "--z3timeout 10"
-#set-options "--lax" // OK
-
-val multiplication_step_p1: a:bigint -> b:bigint -> ctr:u32{w ctr<norm_length} -> 
-  c:bigint{disjoint a c /\ disjoint b c /\ length c >= 2*norm_length-1} -> 
-  tmp:bigint{disjoint a tmp /\ disjoint b tmp /\ disjoint c tmp} ->  STL unit 
-     (requires (fun h -> (bound27 h a) /\ (norm h b) /\ (live h c) /\ (live h tmp)
-        /\ (maxValue h c (length c) <= w ctr * pow2 53)
-	/\ (eval h c (2*norm_length-1) = eval h a (norm_length) * eval h b (w ctr)) ))
-     (ensures (fun h0 u h1 -> (bound27 h0 a) /\ (norm h0 b) /\ (live h0 c) /\ (live h0 tmp)       
-       /\ (bound27 h1 a) /\ (norm h1 b) /\ (live h1 c) /\ (live h1 tmp) /\ (modifies_2 c tmp h0 h1)
-       /\ (maxValue h0 c (length c) <= w ctr * pow2 53)
-       /\ (maxValue h1 c (length c) <= (w ctr+1) * pow2 53)
-       /\ (eval h0 c (2*norm_length-1) = eval h0 a (norm_length) * eval h0 b (w ctr))
-       /\ (eval h1 c (2*norm_length-1) = eval h0 c (2*norm_length-1) + pow2 (bitweight templ (w ctr)) * eval h0 a norm_length * v (get h0 b (w ctr))) ))
-let multiplication_step_p1 a b ctr c tmp =
-  let h0 = HST.get() in
-  multiplication_step_0 a b ctr c tmp;
-  let h1 = HST.get() in
-  (* eq_lemma_1 h0 h1 tmp a; *)
-  (* eq_lemma_1 h0 h1 tmp b;   *)
-  (* eq_lemma_1 h0 h1 tmp c;   *)
-  multiplication_step_lemma_001 h0 h1 a b (w ctr) c tmp; 
-  fsum_index c ctr tmp 0ul nlength 0ul;
-  let h2 = HST.get() in 
-  (* eq_lemma_1 h1 h2 c a; *)
-  (* eq_lemma_1 h1 h2 c b; *)
-  (* eq_lemma_1 h1 h2 c tmp; *)
-  lemma_helper_70 h1 h2 ctr c;
-  multiplication_step_lemma_02 h0 h1 h2 a b (w ctr) c tmp
-
-#reset-options
-
-let helper_lemma_61 (a:int) (b:int) (c:int) (d:int) : Lemma (a*b*c+d = d+c*a*b) = ()
-
-val helper_lemma_6: h0:heap -> h1:heap -> a:bigint -> b:bigint -> ctr:nat{ctr < norm_length} -> 
-  c:bigint{disjoint a c /\ disjoint b c /\ length c >= 2 * norm_length - 1} -> 
-  tmp:bigint{disjoint a tmp /\ disjoint b tmp /\ disjoint c tmp} -> Lemma 
-     (requires (bound27 h0 a /\ norm h0 b /\ live h0 c))
-    (ensures (bound27 h0 a /\ norm h0 b /\ live h0 c
-       /\ eval h0 c (2*norm_length-1) + pow2 (bitweight templ ctr) * eval h0 a (norm_length) * v (get h0 b ctr)  = eval h0 a (norm_length) * v (get h0 b ctr) * pow2 (bitweight templ ctr) + eval h0 c (2*norm_length-1) ))
-let helper_lemma_6 h0 h1 a b ctr c tmp = 
-  helper_lemma_61 (eval h0 a norm_length) (v (get h0 b ctr)) (pow2 (bitweight templ ctr)) (eval h0 c (2*norm_length-1))
-
-val multiplication_step: a:bigint -> b:bigint -> ctr:u32{w ctr < norm_length} -> 
-  c:bigint{disjoint a c /\ disjoint b c /\ length c >= 2*norm_length-1} -> 
-  tmp:bigint{disjoint a tmp /\ disjoint b tmp /\ disjoint c tmp} -> STL unit  
-     (requires (fun h -> bound27 h a /\ norm h b /\ live h c /\ live h tmp
-	/\ maxValue h c (length c) <= w ctr * pow2 53
-	/\ eval h c (2*norm_length-1) = eval h a (norm_length) * eval h b (w ctr)  ))
-     (ensures (fun h0 u h1 -> bound27 h0 a /\ bound27 h1 a /\ norm h0 b /\ norm h1 b
-       /\ live h0 c /\ live h1 c  /\ live h0 tmp /\ live h1 tmp /\ modifies_2 c tmp h0 h1
-       /\ maxValue h0 c (length c) <= w ctr * pow2 53
-       /\ maxValue h1 c (length c) <= (w ctr+1) * pow2 53
-       /\ eval h0 c (2*norm_length-1) = eval h0 a (norm_length) * eval h0 b (w ctr)
-       /\ eval h1 c (2*norm_length-1) = eval h0 a (norm_length) * v (get h0 b (w ctr)) * pow2 (bitweight templ (w ctr)) + eval h0 c (2*norm_length-1) ))
-let multiplication_step a b ctr c tmp =
-  let h0 = HST.get() in
-  multiplication_step_p1 a b ctr c tmp;
-  let h1 = HST.get() in
-  helper_lemma_6 h0 h1 a b (w ctr) c tmp;
-  ()
-
-#reset-options "--z3timeout 20"
-#set-options "--lax" // OK
-
-val multiplication_step_lemma_03: h0:heap -> h1:heap -> a:bigint{norm h0 a} -> 
-  b:bigint{norm h0 b} -> ctr:pos{ctr<=norm_length} -> 
-  c:bigint{live h1 c /\ length c >= 2*norm_length-1} -> Lemma 
-    (requires (eval h1 c (2*norm_length-1) = (eval h0 a (norm_length) * v (get h0 b (norm_length - ctr))) * pow2 (bitweight templ (norm_length - ctr)) + eval h0 a (norm_length) * eval h0 b (norm_length - ctr) ))
-    (ensures ( eval h1 c (2*norm_length-1) = eval h0 a (norm_length) * eval h0 b (norm_length - ctr + 1)))
-let multiplication_step_lemma_03 h0 h1 a b ctr c = 
-  let t = templ in 
-  paren_mul_left (eval h0 a norm_length) (v (get h0 b (norm_length - ctr))) (pow2 (bitweight t (norm_length - ctr))); 
-  cut (eval h1 c (2*norm_length-1) = eval h0 a norm_length * v (get h0 b (norm_length - ctr)) * pow2 (bitweight t (norm_length - ctr)) + eval h0 a norm_length * eval h0 b (norm_length - ctr) );
-  cut (eval h1 c (2*norm_length-1) = eval h0 a norm_length * pow2 (bitweight t (norm_length - ctr)) * v (get h0 b (norm_length - ctr)) + eval h0 a norm_length * eval h0 b (norm_length - ctr) );
-  distributivity_add_right (eval h0 a norm_length) (pow2 (bitweight t (norm_length - ctr)) * v (get h0 b (norm_length - ctr))) (eval h0 b (norm_length - ctr));
-  cut (eval h1 c (2*norm_length-1) = eval h0 a norm_length * (pow2 (bitweight t (norm_length - ctr)) * v (get h0 b (norm_length - ctr)) + eval h0 b (norm_length - ctr)))
-
-#reset-options
-
-val helper_lemma_12: a:nat -> v:nat -> p:nat -> b:nat -> Lemma (a * v * p + (a * b) = a * (p * v + b))
-let helper_lemma_12 a v p b = ()
-
-#reset-options "--z3timeout 100"
-#set-options "--lax" // OK
-
-val multiplication_aux_lemma: h0:heap -> h1:heap -> a:bigint -> b:bigint -> 
-  ctr:pos{ctr <= norm_length} ->  c:bigint{disjoint a c /\ disjoint b c} -> 
-  tmp:bigint{disjoint a tmp /\ disjoint b tmp /\ disjoint c tmp} -> Lemma
-    (requires (bound27 h0 a /\ bound27 h1 a /\ norm h0 b /\ norm h1 b 
-       /\ live h0 c /\ live h1 c /\ live h0 tmp /\ live h1 tmp
-       /\ length c >= 2 * norm_length - 1 /\ modifies_2 c tmp h0 h1
-       /\ maxValue h0 c (length c) <= (norm_length - ctr) * pow2 53
-       /\ maxValue h1 c (length c) <= ((norm_length - ctr)+1) * pow2 53
-       /\ eval h0 c (2*norm_length-1) = eval h0 a (norm_length) * eval h0 b (norm_length - ctr)
-       /\ eval h1 c (2*norm_length-1) = eval h0 a (norm_length) * v (get h0 b (norm_length - ctr)) * pow2 (bitweight templ (norm_length - ctr)) + eval h0 c (2*norm_length-1) ))
-    (ensures (bound27 h1 a /\ norm h1 b /\ live h1 c /\ live h1 tmp
-	/\ length c >= 2 * norm_length - 1
-	/\ maxValue h1 c (length c) <= (norm_length - ctr + 1) * pow2 53
-	/\ eval h1 c (2*norm_length-1) = eval h1 a (norm_length) * eval h1 b (norm_length - ctr + 1) ))
-let multiplication_aux_lemma h0 h1 a b ctr c tmp =
-  (* eq_lemma_2 h0 h1 c tmp a; *)
-  (* eq_lemma_2 h0 h1 c tmp b; *)
-  eval_eq_lemma h0 h1 a a norm_length;
-  eval_eq_lemma h0 h1 b b norm_length;
-  eval_eq_lemma h0 h1 b b (norm_length - ctr);
-  eval_eq_lemma h0 h1 b b (norm_length - ctr + 1); 
-  cut((norm_length - ctr)+1 = norm_length - ctr + 1); 
-  cut(eval h0 a norm_length = eval h1 a norm_length);
-  cut(eval h0 b (norm_length-ctr) = eval h1 b (norm_length - ctr));
-  cut(eval h0 b (norm_length - ctr + 1) = eval h1 b (norm_length - ctr + 1));
-  cut(v (get h0 b (norm_length - ctr)) = v (get h1 b (norm_length - ctr)));
-  helper_lemma_12 (eval h0 a norm_length) (v (get h0 b (norm_length - ctr))) (pow2 (bitweight templ (norm_length - ctr))) (eval h0 b (norm_length - ctr))
-
-#reset-options "--z3timeout 20"
-#set-options "--lax" // OK
-
-val multiplication_aux_lemma_2: h0:heap -> h1:heap -> h2:heap -> a:bigint -> b:bigint -> 
-  ctr:nat{ctr <= norm_length} -> c:bigint{disjoint a c /\ disjoint b c /\ length c >= 2*norm_length-1} -> 
-  tmp:bigint{disjoint a tmp /\ disjoint b tmp /\ disjoint c tmp} -> Lemma 
-    (requires (bound27 h0 a /\ norm h0 b /\ live h1 c /\ live h1 tmp /\ live h0 tmp /\ live h0 c
-       /\ bound27 h1 a /\ norm h1 b /\ live h1 c /\ live h1 tmp
-       /\ bound27 h2 a /\ norm h2 b /\ live h2 c /\ live h2 tmp
-       /\ modifies_2 c tmp h1 h2 /\ modifies_2 c tmp h0 h1
-       /\ eval h2 c (2*norm_length-1) = eval h1 a (norm_length) * eval h1 b (norm_length) ))
-    (ensures (bound27 h0 a /\ norm h0 b /\ live h1 c /\ bound27 h2 a /\ norm h2 b /\ live h2 c
-       /\ modifies_2 c tmp h0 h2
-       /\ eval h2 c (2*norm_length-1) = eval h0 a (norm_length) * eval h0 b (norm_length) ))
-let multiplication_aux_lemma_2 h0 h1 h2 a b ctr c tmp =
-  lemma_modifies_2_trans c tmp h0 h1 h2;
-  (* eq_lemma_2 h0 h1 c tmp a; *)
-  (* eq_lemma_2 h0 h1 c tmp b; *)
-  eval_eq_lemma h0 h1 a a norm_length; 
-  eval_eq_lemma h0 h1 b b norm_length
-
-#reset-options "--z3timeout 100"
-#set-options "--lax" // OK
-
-val multiplication_aux: a:bigint -> b:bigint -> ctr:u32{w ctr<=norm_length} -> 
-  c:bigint{disjoint a c /\ disjoint b c /\ length c >= 2*norm_length-1} -> 
-  tmp:bigint{disjoint a tmp /\ disjoint b tmp /\ disjoint c tmp} -> STL unit
-     (requires (fun h -> bound27 h a /\ norm h b /\ live h c /\ live h tmp
-	/\ maxValue h c (length c) <= (norm_length - w ctr) * pow2 53
-	/\ eval h c (2*norm_length-1) = eval h a (norm_length) * eval h b (norm_length - w ctr) ))
-     (ensures (fun h0 u h1 -> bound27 h0 a /\ norm h0 b /\ live h0 c /\ live h0 tmp
-       /\ bound27 h1 a /\ norm h1 b /\ live h1 c /\ live h1 tmp /\ modifies_2 c tmp h0 h1
-       /\ eval h1 c (2*norm_length-1) = eval h0 a (norm_length) * eval h0 b (norm_length)
-       /\ maxValue h1 c (length c) <= norm_length * pow2 53 ))
-let rec multiplication_aux a b ctr c tmp = 
-  let h0 = HST.get() in
-  if U32.eq ctr 0ul then admit()
-  else begin
-    multiplication_step a b (nlength -| ctr) c tmp; 
-    let h1 = HST.get() in    
-    multiplication_aux_lemma h0 h1 a b (w ctr) c tmp;
-    multiplication_aux a b (ctr-|1ul) c tmp; 
-    let h2 = HST.get() in
-    multiplication_aux_lemma_2 h0 h1 h2 a b (w ctr) c tmp;
-    ()
-  end
-
-#reset-options
-
-val helper_lemma_13: h0:heap -> h1:heap -> a:bigint ->
-  Lemma 
-    (requires (bound27 h0 a /\ modifies_0 h0 h1))
-    (ensures (bound27 h0 a /\ bound27 h1 a /\ live h1 a /\ eval h0 a norm_length = eval h1 a norm_length))
-let helper_lemma_13 h0 h1 a =  
-  (* eq_lemma_0 h0 h1 a; *)
-  eval_eq_lemma h0 h1 a a norm_length;
-  ()
-
-val helper_lemma_131: h0:heap -> h1:heap -> a:bigint ->
-  Lemma 
-    (requires (norm h0 a /\ modifies_0 h0 h1))
-    (ensures (norm h0 a /\ norm h1 a /\ live h1 a /\ eval h0 a norm_length = eval h1 a norm_length))
-let helper_lemma_131 h0 h1 a =  
-  (* eq_lemma_0 h0 h1 a; *)
-  eval_eq_lemma h0 h1 a a norm_length;
-  ()
-
-val helper_lemma_15: h0:heap -> h1:heap -> c:bigint{length c >= 2*norm_length-1} -> Lemma
-    (requires (live h0 c /\ null h0 c /\ modifies_0 h0 h1))
-    (ensures (live h1 c /\ null h1 c /\ maxValue h1 c (length c) = 0 /\ eval h1 c (2*norm_length-1) = 0))
-let helper_lemma_15 h0 h1 c =
-  (* eq_lemma_0 h0 h1 c; *)
-  eval_null h1 c (2*norm_length - 1); 
-  max_value_of_null_lemma h1 c (length c)
-	 
-val multiplication_lemma_1: h0:heap -> h1:heap -> c:bigint{length c >= 2*norm_length-1} -> 
-  a:bigint{disjoint c a} ->  b:bigint{disjoint c b} -> Lemma
-     (requires (bound27 h0 a /\ norm h0 b /\ live h0 c /\ null h0 c /\ modifies_0 h0 h1))
-     (ensures (bound27 h1 a /\ norm h1 b /\ live h1 c /\ null h1 c
-	/\ maxValue h1 c (length c) <= (norm_length - norm_length) * pow2 53
-	/\ eval h1 c (2*norm_length-1) = eval h1 a (norm_length) * eval h1 b (norm_length - norm_length) )) 
-let multiplication_lemma_1 h0 h1 c a b =
-  helper_lemma_13 h0 h1 a;
-  helper_lemma_131 h0 h1 b;
-  helper_lemma_15 h0 h1 c;   
-  cut(eval h1 b 0 = 0)
-
-#reset-options "--z3timeout 100"
-#set-options "--lax" // OK
-val helper_lemma_14: h0:heap -> h1:heap -> h2:heap -> c:bigint -> tmp:bigint{disjoint c tmp} ->
-  Lemma
-    (requires (live h0 c /\ live h2 c /\ ~(contains h0 tmp) /\ modifies_0 h0 h1 /\ live h1 tmp /\ modifies_2 c tmp h1 h2))
-    (ensures ((frameOf tmp = frameOf c /\ modifies_1 c h0 h2)
-	      \/ (frameOf tmp <> frameOf c /\ modifies_bufs (frameOf c) (only c) h0 h2
-		  /\ modifies_bufs (frameOf tmp) TSet.empty h0 h2)))
-let helper_lemma_14 h0 h1 h2 c tmp = 
-  if frameOf tmp = frameOf c then begin
-    let rid = frameOf tmp in
-    cut(modifies_bufs rid TSet.empty h0 h1);
-    cut(modifies_bufs rid (only c ++ only tmp) h1 h2);
-    cut(~(contains h0 tmp));
-    cut(modifies_bufs rid (only c) h0 h2)
-  end
-  else ()
-
-#reset-options
-#set-options "--lax" // OK
-
-val multiplication_lemma_2: h0:heap -> h1:heap -> h2:heap -> c:bigint{length c >= 2*norm_length-1} -> 
-  a:bigint{disjoint c a} -> b:bigint{disjoint c b} -> 
-  tmp:bigint{disjoint a tmp /\ disjoint b tmp /\ disjoint c tmp} -> Lemma
-     (requires (bound27 h0 a /\ norm h0 b /\ live h0 c /\ null h0 c
-	/\ modifies_0 h0 h1 /\ ~(contains h0 tmp) /\ live h1 tmp /\ frameOf tmp = h0.tip
-	/\ bound27 h1 a /\ norm h1 b /\ live h1 c /\ null h1 c
-	/\ maxValue h1 c (length c) <= (norm_length - norm_length) * pow2 53
-	/\ eval h1 c (2*norm_length-1) = eval h1 a (norm_length) * eval h1 b (norm_length - norm_length)
-        /\ bound27 h2 a /\ norm h2 b /\ live h2 c
-        /\ modifies_2 c tmp h1 h2
-        /\ eval h2 c (2*norm_length-1) = eval h1 a (norm_length) * eval h1 b (norm_length)
-        /\ maxValue h2 c (length c) <= norm_length * pow2 53 ))
-     (ensures (bound27 h0 a /\ norm h0 b /\ live h0 c /\ bound27 h2 a /\ norm h2 b /\ live h2 c
-       /\ modifies_2_1 c h0 h2
-       /\ ((frameOf tmp = frameOf c /\ modifies_1 c h0 h2)
-	      \/ (frameOf tmp <> frameOf c /\ modifies_bufs (frameOf c) (only c) h0 h2
-		  /\ modifies_bufs (frameOf tmp) TSet.empty h0 h2))
-       /\ eval h2 c (2*norm_length-1) = eval h0 a (norm_length) * eval h0 b (norm_length)
-       /\ maxValue h2 c (length c) <= norm_length * pow2 53 ))
-let multiplication_lemma_2 h0 h1 h2 c a b tmp =
-  lemma_modifies_2_1 c tmp h0 h1 h2;
-  helper_lemma_14 h0 h1 h2 c tmp; 
-  helper_lemma_13 h0 h1 a;
-  helper_lemma_13 h0 h1 b
-
-let lemma_mult_0 h0 h1 (a:bigint) (c:bigint) : Lemma
-  (requires (bound27 h0 a /\ disjoint a c /\ modifies_1 c h0 h1 /\ live h0 c))
-  (ensures  (bound27 h1 a))
-  = ()(* eq_lemma_1 h0 h1 c a *)
-
-let lemma_mult_1 h0 h1 (a:bigint) (c:bigint) : Lemma
-  (requires (norm h0 a /\ disjoint a c /\ modifies_1 c h0 h1 /\ live h0 c))
-  (ensures  (norm h1 a))
-  = () (* eq_lemma_1 h0 h1 c a *)
-
-let lemma_mult_2 h0 h1 (c:bigint{length c >= 2*norm_length-1}) : Lemma
-  (requires (live h0 c /\ frameOf c <> h0.tip /\ popped h0 h1))
-  (ensures  (live h0 c /\ live h1 c /\ maxValue h1 c (length c) = maxValue h0 c (length c) /\ eval h1 c (2*norm_length-1) = eval h0 c (2*norm_length-1) ))
-  = (* eq_lemma_popped h0 h1 c;  *)
-    eval_eq_lemma h0 h1 c c (2*norm_length-1);
-    maxValue_eq_lemma h0 h1 c c (length c)
-
-#reset-options "--z3timeout 100"
-#set-options "--lax" // OK
-
-(* Code : core multiplication function *)
-val multiplication: c:bigint{length c >= 2*norm_length-1} -> a:bigint{disjoint c a} -> 
-  b:bigint{disjoint c b} -> STL unit
+  let a0 = a.(0ul) in
+  let a1 = a.(1ul) in
+  let a2 = a.(2ul) in
+  let a3 = a.(3ul) in
+  let a4 = a.(4ul) in
+  a.(0ul) <- a0 *^ s;
+  a.(1ul) <- a1 *^ s;
+  a.(2ul) <- a2 *^ s;
+  a.(3ul) <- a3 *^ s;
+  a.(4ul) <- a4 *^ s
+
+assume new type bound27 (h:mem) (a:bigint)
+
+val multiplication: c:bigint -> a:bigint{disjoint c a} -> b:bigint{disjoint c b} -> Stack unit
      (requires (fun h -> bound27 h a /\ norm h b /\ live h c /\ null h c))
-     (ensures (fun h0 u h1 -> bound27 h0 a /\ norm h0 b /\ live h0 c /\ bound27 h1 a /\ norm h1 b /\ live h1 c
+     (ensures (fun h0 u h1 -> bound27 h0 a /\ norm h0 b /\ live h1 c
        /\ modifies_1 c h0 h1
-       /\ eval h1 c (2*norm_length-1) = eval h0 a (norm_length) * eval h0 b (norm_length)
-       /\ maxValue h1 c (length c) <= norm_length * pow2 53 ))
+       (* /\ eval h1 c (2*norm_length-1) = eval h0 a (norm_length) * eval h0 b (norm_length) *)
+       (* /\ maxValue h1 c (length c) <= norm_length * pow2 53 *)
+     ))
 let multiplication c a b =
-  let hinit = HST.get() in
-  push_frame ();
-  let h0 = HST.get() in
-  (* eq_lemma_fresh hinit h0 a; *)
-  (* eq_lemma_fresh hinit h0 b; *)
-  (* eq_lemma_fresh hinit h0 c; *)
-  eval_eq_lemma hinit h0 a a norm_length;
-  eval_eq_lemma hinit h0 b b norm_length;
-  let tmp = create 0UL nlength in 
-  let h1 = HST.get() in
-  (* eq_lemma_0 h0 h1 a;  *)
-  (* eq_lemma_0 h0 h1 b;  *)
-  (* eq_lemma_0 h0 h1 c; *)
-  multiplication_lemma_1 h0 h1 c a b;
-  multiplication_aux a b nlength c tmp; 
-  let h2 = HST.get() in 
-  multiplication_lemma_2 h0 h1 h2 c a b tmp;
-  pop_frame ();
-  let hfin = HST.get() in
-  modifies_popped_1 c hinit h0 h2 hfin;  
-  (* eq_lemma_popped h2 hfin c; *)
-  lemma_mult_0 hinit hfin a c;
-  lemma_mult_1 hinit hfin b c;
-  lemma_mult_2 h2 hfin c
+  let a0 = a.(0ul) in let a1 = a.(1ul) in let a2 = a.(2ul) in let a3 = a.(3ul) in let a4 = a.(4ul) in
+  let b0 = b.(0ul) in let b1 = b.(1ul) in let b2 = b.(2ul) in let b3 = b.(3ul) in let b4 = b.(4ul) in
+  let ab00 = a0 *^ b0 in
+  let ab01 = a0 *^ b1 in
+  let ab02 = a0 *^ b2 in
+  let ab03 = a0 *^ b3 in
+  let ab04 = a0 *^ b4 in
+  let ab10 = a1 *^ b0 in
+  let ab11 = a1 *^ b1 in
+  let ab12 = a1 *^ b2 in
+  let ab13 = a1 *^ b3 in
+  let ab14 = a1 *^ b4 in
+  let ab20 = a2 *^ b0 in
+  let ab21 = a2 *^ b1 in
+  let ab22 = a2 *^ b2 in
+  let ab23 = a2 *^ b3 in
+  let ab24 = a2 *^ b4 in
+  let ab30 = a3 *^ b0 in
+  let ab31 = a3 *^ b1 in
+  let ab32 = a3 *^ b2 in
+  let ab33 = a3 *^ b3 in
+  let ab34 = a3 *^ b4 in
+  let ab40 = a4 *^ b0 in
+  let ab41 = a4 *^ b1 in
+  let ab42 = a4 *^ b2 in
+  let ab43 = a4 *^ b3 in
+  let ab44 = a4 *^ b4 in
+  let c0 = ab00 in
+  let c1 = ab01 +^ ab10 in
+  let c2 = ab02 +^ ab11 +^ ab20 in
+  let c3 = ab03 +^ ab12 +^ ab21 +^ ab30 in
+  let c4 = ab04 +^ ab13 +^ ab22 +^ ab31 +^ ab40 in
+  let c5 = ab14 +^ ab23 +^ ab32 +^ ab41 in
+  let c6 = ab24 +^ ab33 +^ ab42 in
+  let c7 = ab34 +^ ab43 in
+  let c8 = ab44 in
+  c.(0ul) <- c0;
+  c.(1ul) <- c1;
+  c.(2ul) <- c2;
+  c.(3ul) <- c3;
+  c.(4ul) <- c4;
+  c.(5ul) <- c5;
+  c.(6ul) <- c6;
+  c.(7ul) <- c7;
+  c.(8ul) <- c8
 
-#reset-options
+val times_5: b:U64.t -> Tot (b':U64.t)
+let times_5 b = (b <<^ 2ul) +^ b
 
-(*** Modulo ***)
+val freduce_degree: b:bigint -> Stack unit
+  (requires (fun h -> live h b
+    (* /\ satisfiesModuloConstraints h b *)
+  ))
+  (ensures (fun h0 _ h1 -> live h0 b /\ live h1 b /\ modifies_1 b h0 h1
+    (* /\ satisfiesModuloConstraints h0 b *)
+    (* /\ (forall (i:nat). {:pattern (v (get h1 b i))} i <= norm_length ==> *)
+    (* 	v (get h1 b i) < pow2 63) *)
+    (* /\ eval h1 b norm_length % reveal prime = eval h0 b (2*norm_length-1) % reveal prime *)
+  ))
+let freduce_degree b =
+  let b0 = b.(0ul) in
+  let b1 = b.(1ul) in
+  let b2 = b.(2ul) in
+  let b3 = b.(3ul) in
+  let b5 = b.(5ul) in
+  let b6 = b.(6ul) in
+  let b7 = b.(7ul) in
+  let b8 = b.(8ul) in
+  let b0' = b0 +^ times_5 b5 in
+  let b1' = b1 +^ times_5 b6 in
+  let b2' = b2 +^ times_5 b7 in
+  let b3' = b3 +^ times_5 b8 in
+  b.(0ul) <- b0';
+  b.(1ul) <- b1';
+  b.(2ul) <- b2';
+  b.(3ul) <- b3'
 
-(* Immediately comes from the modulo definition *)
-val prime_modulo_lemma: unit -> Lemma (pow2 130 % (reveal prime) = 5)
-let prime_modulo_lemma () = assert_norm ((pow2 130 % (reveal prime) = 5))
+val mod2_26: U64.t -> Tot U64.t
+let mod2_26 x = x &^ 0x3ffffffuL
 
+val div2_26: U64.t -> Tot U64.t
+let div2_26 x = x >>^ 26ul
 
-val modulo_lemma: a:nat -> b:pos -> Lemma (requires (a < b)) (ensures (a % b = a)) 
-  [SMTPat (a % b)]
-let modulo_lemma a b = ()
-
-let satisfiesModuloConstraints (h:heap) (b:bigint) : GTot Type0 = 
-  live h b /\ length b >= 2*norm_length-1 && maxValue h b (2*norm_length-1) * 6 < pow2 63
-
-val satisfiesModuloConstraints_after_multiplication: h:heap -> b:bigint{live h b /\ length b >= 2*norm_length-1 /\ maxValue h b (length b) <= norm_length * pow2 53} -> Lemma
-  (satisfiesModuloConstraints h b)
-let satisfiesModuloConstraints_after_multiplication h b =
-  maxValue_increases h b (2*norm_length-1) (length b);
-  assert_norm (30 * pow2 53 < pow2 63)
-
-val times_5: x:u64{5 * v x < pow2 64} -> Tot (y:u64{v y = 5 * v x})
-let times_5 x = 
-  let z = x <<^ 2ul in
-  x +^ z
-  
-let reducible (h:heap) (b:bigint) (ctr:nat{ctr < norm_length-1}) : GTot Type0 =
-  live h b /\ length b >= 2*norm_length-1 
-  /\ (forall (i:nat). {:pattern (get h b (i+norm_length))}
-      i <= ctr ==> v (get h b i) + 5 * v (get h b (i+norm_length)) < pow2 64)
-
-let times5 (h0:heap) (h1:heap) (b:bigint) (ctr:nat{ctr < norm_length - 1}) : GTot Type0 =
-  live h0 b /\ live h1 b /\ length b >= 2*norm_length-1
-  /\ (forall (i:nat). {:pattern (get h1 b i)}
-       i <= ctr ==> v (get h1 b i) = v (get h0 b i) + 5 * (v (get h0 b (i+norm_length))))
-
-let untouched (h0:heap) (h1:heap) (b:bigint) (ctr:nat) : GTot Type0 = 
-  live h0 b /\ live h1 b /\ length b >= 2*norm_length-1
-  /\ (forall (i:nat). {:pattern (get h1 b i)} (i > ctr /\ i < 2*norm_length-1) ==> 
-      get h0 b i = get h1 b i)
-
-#reset-options "--z3timeout 100"
-#set-options "--lax" // OK
-
-val pow2_bitweight_lemma_1: ctr:pos -> Lemma
-  (pow2 (bitweight templ (ctr+norm_length-1)) =
-   pow2 (bitweight templ (ctr-1)) * pow2 (bitweight templ norm_length))
-let rec pow2_bitweight_lemma_1 ctr =
-  match ctr with
-  | 1 -> ()
-  | _ -> 
-    cut(ctr-1+norm_length = ctr+norm_length-1 /\ ctr+norm_length-1 = (ctr-1) + norm_length
-	/\ (ctr+norm_length-1)-1=ctr+norm_length-2); 
-    pow2_bitweight_lemma_1 (ctr-1); 
-    cut (pow2 (bitweight templ (ctr+norm_length-2)) = pow2 (bitweight templ (ctr-2)) * pow2 (bitweight templ norm_length)); 
-    cut (bitweight templ (ctr+norm_length-1) = bitweight templ (ctr+norm_length-2) + 26); 
-    Math.Lemmas.pow2_plus (bitweight templ (ctr+norm_length-2)) 26;
-    cut(pow2 (bitweight templ (ctr+norm_length-1)) = pow2 26 * pow2 (bitweight templ (ctr+norm_length-2))); 
-    cut(pow2 (bitweight templ (ctr+norm_length-1)) = pow2 26 * (pow2 (bitweight templ (ctr-2)) * pow2 (bitweight templ norm_length)));  
-    paren_mul_right (pow2 26) (pow2 (bitweight templ (ctr-2))) (pow2 (bitweight templ norm_length));
-    cut (pow2 (bitweight templ (ctr+norm_length-1)) = pow2 26 * pow2 (bitweight templ (ctr-2)) * pow2 (bitweight templ norm_length)); 
-    Math.Lemmas.pow2_plus 26 (bitweight templ (ctr-2));
-    cut (pow2 (bitweight templ (ctr+norm_length-1)) = pow2 (26 + bitweight templ (ctr-2)) * pow2 (bitweight templ norm_length)) 
-
-#reset-options
-
-val bitweight_norm_length_lemma: unit -> Lemma 
-  (requires True)
-  (ensures (bitweight templ norm_length = 130))
-  [SMTPat (bitweight templ norm_length)]
-let bitweight_norm_length_lemma () = 
-  assert_norm (bitweight templ norm_length = 130)
-
-(* TODO: express in terms of general % property *)
-assume val helper_lemma_5: a:nat -> b:nat -> c:nat -> p:pos -> Lemma (ensures ( (a*b+c) % p = ((a % p) * b + c)%p))
-
-val lemma_aux_0: a:int -> b:int -> c:int -> d:int -> Lemma (a * b + c - (a * (b + 5 * d) + c) = - 5 * a * d)
-let lemma_aux_0 a b c d = ()
-
-#reset-options "--z3timeout 10"
-#set-options "--lax" // OK
-
-val freduce_degree_lemma_021: h0:heap -> h1:heap -> b:bigint{live h1 b /\ live h0 b /\ length b >= 2 * norm_length - 1} -> ctr:pos{ctr < norm_length-1} -> Lemma
-    (requires ((forall (i:nat). {:pattern (get h1 b i)}
-	(i < length b /\ i <> ctr) ==> get h1 b i = get h0 b i) 
-	/\ v (get h1 b ctr) = v (get h0 b ctr) + 5 * v (get h0 b (ctr+norm_length)) ))
-    (ensures (eval h0 b (norm_length+1+ctr) = (pow2 130 * pow2 (bitweight templ ctr)) * v (get h0 b (norm_length+ctr)) + eval h0 b (norm_length+ctr)))
-let freduce_degree_lemma_021 h0 h1 b ctr = 
-  let prime = reveal prime in 
-  cut (ctr+norm_length = norm_length+ctr /\ (norm_length+1+ctr)-1 = norm_length + ctr /\ norm_length+ctr = (ctr+1)+norm_length-1); 
-  cut (eval h0 b (norm_length+1+ctr) = pow2 (bitweight templ (norm_length+ctr)) * v (get h0 b (norm_length+ctr)) + eval h0 b (ctr+norm_length)); 
-  pow2_bitweight_lemma_1 (ctr+1); 
-  cut(pow2 (bitweight templ (norm_length+ctr)) = pow2 130 * pow2 (bitweight templ ctr)); 
-  paren_mul_left (pow2 130) (pow2 (bitweight templ ctr)) (v (get h0 b (norm_length+ctr))); 
-  paren_mul_right (pow2 130) (pow2 (bitweight templ ctr)) (v (get h0 b (norm_length+ctr)))
-
-#reset-options "--z3timeout 50"
-#set-options "--lax" // OK
-
-val freduce_degree_lemma_022: h0:heap -> h1:heap -> b:bigint{live h1 b /\ live h0 b /\ length b >= 2 * norm_length - 1} -> ctr:pos{ctr < norm_length-1} -> Lemma
-    (requires ((forall (i:nat). {:pattern (get h1 b i)}
-	(i < length b /\ i <> ctr) ==> get h1 b i = get h0 b i)
-	/\ v (get h1 b ctr) = v (get h0 b ctr) + 5 * v (get h0 b (ctr+norm_length)) 
-	))
-    (ensures (eval h0 b (norm_length+ctr) - eval h0 b (ctr+1) = eval h1 b (norm_length+ctr) - eval h1 b (ctr+1)))
-let freduce_degree_lemma_022 h0 h1 b ctr =
-  cut (forall (i:nat). (i < length b /\ i >= ctr+1) ==> get h1 b i = get h0 b i);
-  cut (forall (i:nat). (ctr+1) + (i - ctr -1) = i);
-  cut (forall (i:nat). i < norm_length + ctr - (ctr + 1) ==> get h1 b (ctr+1+i) = get h0 b (ctr+1+i));
-  eval_partial_eq_lemma h0 h1 b b (ctr+1) (norm_length+ctr);
-  cut (eval h0 b (norm_length+ctr) - eval h0 b (ctr+1) = eval h1 b (norm_length+ctr) - eval h1 b (ctr+1))
-
-#reset-options "--z3timeout 10"
-
-let lemma_aux_000 (a:nat) (b:nat) : Lemma (a * b >= 0) = ()
-
-#reset-options "--z3timeout 200"
-#set-options "--lax" // OK
-
-val freduce_degree_lemma_2: h0:heap -> h1:heap -> b:bigint{live h1 b /\ live h0 b /\ length b >= 2 * norm_length - 1} -> ctr:pos{ctr < norm_length-1} -> Lemma
-    (requires ((forall (i:nat). {:pattern (get h1 b i)}
-	(i < length b /\ i <> ctr) ==> get h1 b i = get h0 b i)
-	/\ v (get h1 b ctr) = v (get h0 b ctr) + 5 * v (get h0 b (ctr+norm_length)) ))
-    (ensures (eval h0 b (norm_length+1+ctr) % (reveal prime) = eval h1 b (norm_length+ctr) % (reveal prime)))
-let freduce_degree_lemma_2 h0 h1 b ctr =
-  let prime = reveal prime in  
-  pow2_bitweight_lemma_1 (ctr+1); 
-  paren_mul_left (pow2 130) (pow2 (bitweight templ ctr)) (v (get h0 b (norm_length+ctr)));
-  paren_mul_right (pow2 130) (pow2 (bitweight templ ctr)) (v (get h0 b (norm_length+ctr)));
-  freduce_degree_lemma_021 h0 h1 b ctr;
-  lemma_aux_000 (pow2 (bitweight templ ctr)) (v (get h0 b (norm_length+ctr)));
-  helper_lemma_5 (pow2 130) (pow2 (bitweight templ ctr) * v (get h0 b (norm_length+ctr))) (eval h0 b (norm_length+ctr)) prime;
-  cut (eval h0 b (norm_length+1+ctr) % prime = ((pow2 130 % prime) * pow2 (bitweight templ ctr) * v (get h0 b (norm_length+ctr)) + eval h0 b (norm_length+ctr)) % prime);
-  prime_modulo_lemma ();
-  cut (eval h0 b (norm_length+1+ctr) % prime = (5 * pow2 (bitweight templ ctr) * v (get h0 b (norm_length+ctr)) + eval h0 b (norm_length+ctr)) % prime);
-  freduce_degree_lemma_022 h0 h1 b ctr;
-  eval_eq_lemma h0 h1 b b ctr;
-  eval_def h0 b (ctr+1);
-  eval_def h1 b (ctr+1);
-  cut (eval h0 b (ctr+1) = pow2 (bitweight templ ctr) * v (get h0 b ctr) + eval h0 b ctr);
-  cut (eval h1 b (ctr+1) = pow2 (bitweight templ ctr) * (v (get h0 b ctr) + 5 * v (get h0 b (norm_length+ctr))) + eval h0 b ctr);
-  lemma_aux_0 (pow2 (bitweight templ ctr)) (v (get h0 b ctr)) (eval h0 b ctr) (v (get h0 b (norm_length+ctr)));
-  cut (eval h0 b (ctr+1) - eval h1 b (ctr+1) = - 5 * pow2 (bitweight templ ctr) * v (get h0 b (norm_length+ctr))); 
-  distributivity_add_right (pow2 (bitweight templ ctr)) (v (get h0 b ctr)) (5 * v (get h0 b (norm_length+ctr))); 
-  cut ( eval h0 b (norm_length+1+ctr) % prime = (5 * pow2 (bitweight templ ctr) * v (get h0 b (norm_length+ctr)) + eval h1 b (norm_length+ctr) + eval h0 b (ctr+1) - eval h1 b (ctr+1)) % prime);
-  cut ( eval h0 b (norm_length+1+ctr) % prime = (5 * pow2 (bitweight templ ctr) * v (get h0 b (norm_length+ctr)) + eval h1 b (norm_length+ctr) - 5 * pow2 (bitweight templ ctr) * v (get h0 b (norm_length+ctr))) % prime);
-  cut ( eval h0 b (norm_length+1+ctr) % prime = (eval h1 b (norm_length+ctr) ) % prime)
-
-#reset-options "--z3timeout 200"
-#set-options "--lax" // OK
-
-val freduce_degree_lemma:
-  h0:heap -> h1:heap -> b:bigint{live h1 b /\ live h0 b /\ length b >= 2 * norm_length - 1} -> 
-  ctr:nat{ctr < norm_length-1} -> Lemma
-    (requires ((forall (i:nat). {:pattern (get h1 b i)}
-	(i < length b /\ i <> ctr) ==> get h1 b i = get h0 b i)
-      /\ v (get h1 b ctr) = v (get h0 b ctr) + 5 * v (get h0 b (ctr+norm_length)) ))
-    (ensures (eval h0 b (norm_length+1+ctr) % (reveal prime) = eval h1 b (norm_length+ctr) % (reveal prime)))  
-let freduce_degree_lemma h0 h1 b ctr =
-  let prime = reveal prime in
-  if ctr = 0 then (
-    helper_lemma_5 (pow2 130) (v (get h0 b norm_length)) (eval h0 b norm_length) prime;
-    prime_modulo_lemma ();
-    cut(eval h0 b 1 = v (get h0 b 0) /\ eval h1 b 1 = v (get h0 b 0) + 5 * v (get h0 b norm_length)); 
-    eval_partial_eq_lemma h0 h1 b b 1 norm_length;
-    cut(eval h1 b norm_length - eval h1 b 1 = eval h0 b norm_length - eval h0 b 1)
-  ) else (
-    freduce_degree_lemma_2 h0 h1 b ctr
-  )
-
-#reset-options "--z3timeout 100"
-#set-options "--lax" // OK
-
-val freduce_degree': 
-  b:bigint -> ctr:u32{w ctr < norm_length - 1} -> STL unit 
-    (requires (fun h -> reducible h b (w ctr))) 
-    (ensures (fun h0 _ h1 -> untouched h0 h1 b (w ctr) /\ times5 h0 h1 b (w ctr)
-      /\ eval h1 b (norm_length) % reveal prime = eval h0 b (norm_length+1+w ctr) % reveal prime
-      /\ modifies_1 b h0 h1))
-let rec freduce_degree' b ctr' =
-  let h0 = HST.get() in
-  if U32.eq ctr' 0ul then begin
-    let b5ctr = index b (0ul+|nlength) in 
-    let bctr = index b 0ul in
-    let b5ctr = times_5 b5ctr in
-    let bctr = bctr +^ b5ctr in 
-    upd b 0ul bctr;
-    let h1 = HST.get() in
-    freduce_degree_lemma h0 h1 b 0;
-    cut (eval h0 b (norm_length+1+0) % reveal prime = eval h1 b (norm_length+0) % reveal prime);
-    cut (eval h0 b (norm_length+1) % reveal prime = eval h1 b (norm_length+0) % reveal prime)
-    end
-  else begin
-    let ctr = ctr' in
-    let b5ctr = index b (ctr +| nlength) in 
-    let bctr = index b ctr in
-    let b5ctr = times_5 b5ctr in
-    let bctr = bctr +^ b5ctr in 
-    upd b ctr bctr;
-    let h1 = HST.get() in
-    freduce_degree_lemma h0 h1 b (w ctr); 
-    cut (eval h0 b (norm_length+1+w ctr) % reveal prime = eval h1 b (norm_length+w ctr) % reveal prime);
-    cut(reducible h1 b (w ctr-1)); 
-    freduce_degree' b (ctr-|1ul); 
-    let h2 = HST.get() in 
-    cut (forall (i:nat). {:pattern (v (get h1 b i))} (i > w ctr /\ i < 2*norm_length-1) ==>
-	   v (get h1 b i) = v (get h0 b i)); 
-    cut(untouched h0 h2 b (w ctr));
-    cut (times5 h0 h2 b (w ctr)) ;
-    ()
-  end
-
-#reset-options
-
-val aux_lemma_4': h:heap -> b:bigint -> Lemma
-  (requires (satisfiesModuloConstraints h b))
-  (ensures (reducible h b (norm_length-2)))
-let aux_lemma_4' h b =
-  maxValue_lemma_aux h b (2*norm_length-1);
-  pow2_lt_compat 64 63;
-  ()
-  
-val aux_lemma_5': h0:heap -> h1:heap -> b:bigint -> Lemma
-  (requires (live h0 b /\ satisfiesModuloConstraints h0 b /\ times5 h0 h1 b (norm_length-2)
-      /\ untouched h0 h1 b (norm_length-2)))
-  (ensures (live h0 b /\ satisfiesModuloConstraints h0 b /\ times5 h0 h1 b (norm_length-2)
-    /\ (forall (i:nat). i <= norm_length ==> v (get h1 b i) < pow2 63)))
-let aux_lemma_5' h0 h1 b = 
-  maxValue_lemma_aux h0 b (2*norm_length-1)
-
-val freduce_degree: b:bigint -> STL unit 
-  (requires (fun h -> live h b /\ satisfiesModuloConstraints h b)) 
-  (ensures (fun h0 _ h1 -> live h0 b /\ live h1 b /\ satisfiesModuloConstraints h0 b
-    /\ modifies_1 b h0 h1
-    /\ (forall (i:nat). {:pattern (v (get h1 b i))} i <= norm_length ==> 
-	v (get h1 b i) < pow2 63)
-    /\ eval h1 b norm_length % reveal prime = eval h0 b (2*norm_length-1) % reveal prime))
-let freduce_degree b = 
-  let h0 = HST.get() in
-  aux_lemma_4' h0 b; 
-  freduce_degree' b (nlength-|2ul); 
-  let h1 = HST.get() in
-  aux_lemma_5' h0 h1 b
-
-val pow2_bitweight_lemma: ctr:nat -> Lemma
-  (pow2 (bitweight templ (ctr+1)) =
-   pow2 (bitweight templ ctr) * pow2 (templ ctr))
-let pow2_bitweight_lemma ctr =
-  Math.Lemmas.pow2_plus (bitweight templ ctr) (templ ctr)
-
-val helper_lemma_2: pb:nat -> pc:pos -> a0:nat -> b:nat ->
-  Lemma ((pb * pc) * a0/pc + (pb * (a0 % pc) + b) = pb * a0 + b)
-let helper_lemma_2 pb pc a0 b = ()
-
-#reset-options "--z3timeout 10"
-//#set-options "--lax" // TODO
-
-val lemma_helper_80: ha:heap -> a:bigint{live ha a /\ length a >= norm_length+1} ->
-  hb:heap -> b:bigint{live hb b /\ length b >= norm_length+1} -> ctr:nat{ctr < norm_length} -> Lemma
-    (requires (v (get hb b ctr) = v (get ha a ctr) % pow2 (templ ctr)
-      /\ v (get hb b (ctr+1)) = v (get ha a (ctr+1)) + v (get ha a ctr) / pow2 (templ ctr)
-      /\ (forall (i:nat). {:pattern (get hb b i)}
-	  (i < norm_length+1 /\ i <> ctr /\ i <> ctr+1) ==> get hb b i = get ha a i) ))
-    (ensures (eval hb b (ctr+2) = pow2 (bitweight templ (ctr+1)) * (v (get ha a (ctr+1)) + v (get ha a ctr) / pow2 (templ ctr)) + (pow2 (bitweight templ ctr) * (v (get ha a ctr) % pow2 (templ ctr)) + eval hb b ctr)))
-let lemma_helper_80 ha a hb b ctr = 
-  eval_eq_lemma ha hb a b ctr;
-  eval_def hb b (ctr+2);
-  cut(eval hb b (ctr+2) = pow2 (bitweight templ (ctr+1)) * v (get hb b (ctr+1)) + eval hb b (ctr+1));
-  cut(eval hb b (ctr+2) = pow2 (bitweight templ (ctr+1)) * v (get hb b (ctr+1)) + (pow2 (bitweight templ ctr) * v (get hb b ctr) + eval hb b ctr))
-
-#reset-options "--z3timeout 100"
-
-val eval_carry_lemma: ha:heap -> a:bigint{live ha a /\ length a >= norm_length+1} -> 
-  hb:heap -> b:bigint{live hb b /\ length b >= norm_length+1} -> ctr:nat{ctr < norm_length} -> Lemma
-    (requires (v (get hb b ctr) = v (get ha a ctr) % pow2 (templ ctr)
-      /\ v (get hb b (ctr+1)) = v (get ha a (ctr+1)) + v (get ha a ctr) / pow2 (templ ctr)
-      /\ (forall (i:nat). {:pattern (get hb b i)}
-	  (i < norm_length+1 /\ i <> ctr /\ i <> ctr+1) ==> get hb b i = get ha a i) ))
-    (ensures (eval hb b (norm_length+1) = eval ha a (norm_length+1)))
-let eval_carry_lemma ha a hb b ctr =
-  cut (forall (i:nat). (i < norm_length+1 /\ i >= ctr+2) ==> get hb b i = get ha a i);
-  cut (forall (i:nat). (ctr+2) + (i - ctr -2) = i);
-  cut (forall (i:nat). i < norm_length + 1 - (ctr + 2) ==> get hb b (ctr+2+i) = get ha a (ctr+2+i));
-  eval_partial_eq_lemma ha hb a b (ctr+2) (norm_length+1);
-  eval_eq_lemma ha hb a b ctr;
-  eval_def hb b (ctr+2);
-  (* cut(eval hb b (ctr+2) = pow2 (bitweight templ (ctr+1)) * v (get hb b (ctr+1)) + eval hb b (ctr+1)); *)
-  (* cut(eval hb b (ctr+2) = pow2 (bitweight templ (ctr+1)) * v (get hb b (ctr+1)) + (pow2 (bitweight templ ctr) * v (get hb b ctr) + eval hb b ctr));   *)
-  (* cut(eval hb b (ctr+2) = pow2 (bitweight templ (ctr+1)) * (v (get ha a (ctr+1)) + v (get ha a ctr) / pow2 (templ ctr)) + (pow2 (bitweight templ ctr) * (v (get ha a ctr) % pow2 (templ ctr)) + eval hb b ctr)); admit() *)
-  lemma_helper_80 ha a hb b ctr;
-  distributivity_add_right (pow2 (bitweight templ (ctr+1))) (v (get ha a (ctr+1))) (v (get ha a ctr) / pow2 (templ ctr));
-  cut(eval hb b (ctr+2) = 
-	      pow2 (bitweight templ (ctr+1)) * v (get ha a (ctr+1))
-	      + pow2 (bitweight templ (ctr+1)) * v (get ha a ctr) / pow2 (templ ctr) 
-	      + (pow2 (bitweight templ ctr) * (v (get ha a ctr) % pow2 (templ ctr)) + eval hb b ctr));
-  pow2_bitweight_lemma ctr; 
-  cut(eval hb b (ctr+2) = 
-	      pow2 (bitweight templ (ctr+1)) * v (get ha a (ctr+1)) 
-	      + (pow2 (bitweight templ ctr) * pow2 (templ ctr)) * v (get ha a ctr) / pow2 (templ ctr) 
-	      + (pow2 (bitweight templ ctr) * (v (get ha a ctr) % pow2 (templ ctr)) + eval hb b ctr));
-  helper_lemma_2 (pow2 (bitweight templ ctr)) (pow2 (templ ctr)) (v (get ha a ctr)) (eval hb b ctr); 
-  cut( eval hb b (ctr+2) = 
-	      pow2 (bitweight templ (ctr+1)) * v (get ha a (ctr+1)) 
-	      + (pow2 (bitweight templ ctr) * v (get ha a ctr) + eval hb b ctr));  
-  cut(eval hb b (ctr+2) = eval ha a (ctr+2))
-
-#reset-options
-
-val helper_lemma_4: a:nat -> b:nat -> c:pos -> size:pos{size > c} ->
-  Lemma (requires (a < pow2 (size-1) /\ b < pow2 (size-c)))
-	(ensures (a + b < pow2 size))
-let helper_lemma_4 a b c size = 
-  if size-1 > size - c then begin
-    pow2_lt_compat (size-1) (size-c) ;
-    ()
-    end
-  else ()
-
-val auxiliary_lemma_1': bip1:u64 -> c:u64 -> Lemma
-    (requires (v bip1 < pow2 63 /\ v c < pow2 (64 - 26)))
-    (ensures (v bip1 + v c < pow2 64)) 
-let auxiliary_lemma_1' bip1 c =
-  helper_lemma_4 (v bip1) (v c) 26 64
-
-val auxiliary_lemma_2: bip1:u64 -> c:u64 -> Lemma
-    (requires (v bip1 < pow2 26 /\ v c < pow2 16))
-    (ensures (v bip1 + v c < pow2 27)) 
-let auxiliary_lemma_2 bip1 c =
-  helper_lemma_4 (v bip1) (v c) 11 27
-
-(* TODO: move somewhere more appropriate *)
-assume MaxUint32: FStar.UInt.max_int 32 = 4294967295
-
-val mod2_26: a:u64 -> Tot (b:u64{v b = v a % pow2 26})
-let mod2_26 a = 
-  admit(); // TODO
-  let mask = 1uL <<^ 26ul in
-  pow2_lt_compat 64 26;
-  let mask = mask -^ 1uL in
-  let res = a &^ mask in
-  (* SInt.ulogand_lemma_4 #64 a 26 mask; *)
-  res
-
-let carriable (h:heap) (b:bigint) (ctr:nat{ctr <= norm_length}) : GTot Type0 =
-  live h b /\ length b >= norm_length + 1  
-  /\ (forall (i:nat). {:pattern (v (get h b i))}
-      (i > ctr /\ i <= norm_length) ==> v (get h b i) < pow2 63)
-
-let carried (h1:heap) (b:bigint) (ctr:nat{ctr <= norm_length}) : GTot Type0 =
-  live h1 b /\ length b >= norm_length + 1
-  /\ (forall (i:nat). {:pattern (v (get h1 b i))} i < ctr ==> v (get h1 b i) < pow2 (templ ctr))
-  /\ (ctr <> norm_length ==> v (get h1 b norm_length) = 0)
-  /\ (ctr = norm_length ==> v (get h1 b norm_length) < pow2 38)
-  
-let carried' (h1:heap) (b:bigint) (ctr:nat{ctr <= norm_length}) : GTot Type0 =
-  live h1 b /\ length b >= norm_length + 1
-  /\ (forall (i:nat). {:pattern (v (get h1 b i))} (i >= ctr /\ i < norm_length) ==> v (get h1 b i) < pow2 (templ ctr))
-  /\ v (get h1 b norm_length) < pow2 38
-  
-let untouched_2 (h0:heap) (h1:heap) (b:bigint) (ctr:nat) : GTot Type0 =
-  live h0 b /\ live h1 b /\ length b >= norm_length+1 
-  /\ (forall (i:nat). {:pattern (get h1 b i)}
-      ((i < ctr \/ i >= norm_length+1) /\ i < length b) ==> v (get h0 b i) = v (get h1 b i))
-
-#reset-options "--z3timeout 100"
-#set-options "--lax" // OK
-
-val carry: b:bigint -> ctr:u32{w ctr <= norm_length} -> STL unit
-    (requires (fun h -> carriable h b (w ctr) /\ carried h b (w ctr)))
-    (ensures (fun h0 _ h1 -> carried h1 b norm_length /\ untouched_2 h0 h1 b (w ctr)
-      /\ eval h1 b (norm_length+1) = eval h0 b (norm_length+1)
-      /\ modifies_1 b h0 h1 ))
-let rec carry b i =
-  let h0 = HST.get() in
-  if U32.eq i nlength then admit()
-  else begin 
-    let bi = index b i in
-    let ri = mod2_26 bi in
-    upd b i ri;
-    let h1 = HST.get() in
-    let c = (bi >>^ 26ul) in
-    cut (v c = (v bi) / (pow2 26));
-    pow2_minus 64 26;
-    (* TODO *)
-    assume (v c < pow2 (64 - 26));
-    let bip1 = index b (i+|1ul) in
-    auxiliary_lemma_1' bip1 c;
-    let z = bip1 +^ c in
-    upd b (i+|1ul) z;
-    let h2 = HST.get() in
-    eval_carry_lemma h0 b h2 b (w i);
-    carry b (i+|1ul)
-  end 
-
-#reset-options "--z3timeout 20"
-#set-options "--lax" // OK
-
-val carry_top_to_0: b:bigint -> STL unit
-    (requires (fun h -> carried h b norm_length /\ length b >= 2*norm_length-1
-      /\ v (get h b 0) + 5 * v (get h b norm_length) < pow2 64))
-    (ensures (fun h0 _ h1 -> carried h0 b norm_length /\ carried' h1 b 1
-      /\ eval h1 b norm_length % (reveal prime) = eval h0 b (norm_length+1) % (reveal prime)
-      /\ v (get h1 b 0) = v (get h0 b 0) + 5 * v (get h0 b norm_length)
-      /\ (forall (i:nat). {:pattern (v (get h1 b i))} (i > 0 /\ i < length b) ==> 
-	  v (get h1 b i) = v (get h0 b i))
-      /\ modifies_1 b h0 h1))      
-let carry_top_to_0 b =
-  pow2_lt_compat 64 63;
-  let h0 = HST.get() in
-  let b0 = index b 0ul in
-  let btop = index b nlength in 
-  let btop_5 = times_5 btop in
-  upd b 0ul (b0 +^ btop_5);
-  let h1 = HST.get() in
-  freduce_degree_lemma h0 h1 b 0
-
-#reset-options
-
-let carriable2 (h:heap) (b:bigint) (ctr:pos{ctr<=norm_length}) : GTot Type0 =
-  live h b /\ length b >= norm_length + 1
-  /\ (forall (i:nat). {:pattern (v (get h b i))} i < ctr ==> v (get h b i) < pow2 26)
-  /\ (forall (i:nat). {:pattern (v (get h b i))} (i > ctr /\ i < norm_length) ==> v (get h b i) < pow2 26)
-  /\ (ctr < norm_length ==> v (get h b norm_length) = 0)
-  /\ (ctr = norm_length ==> v (get h b norm_length) < 2)
-  /\ v (get h b ctr) < pow2 26 + pow2 16
-  /\ (v (get h b ctr) >= pow2 26 ==> (
-      forall (i:nat). {:pattern (v (get h b i))} ( i < ctr /\ i > 0) ==> v (get h b i) < pow2 16))
-  /\ ((ctr = norm_length /\ v (get h b norm_length) = 1) ==> 
-      (forall (i:nat). {:pattern (v (get h b i))} (i > 0 /\ i < norm_length) ==> v (get h b i) < pow2 16))
-
-val lemma_aux: a:nat -> b:pos -> Lemma (Math.Lib.div a b > 0 ==> a >= b)
-let lemma_aux a b = 
-  ()
-
-(* TODO: express in terms of % properties *)
-assume val lemma_aux_2: a:u64 -> Lemma ((v a < pow2 26+pow2 16 /\ v a >= pow2 26) ==> v a % pow2 26 < pow2 16)
-
-#reset-options "--z3timeout 100"
-#set-options "--lax" // OK
-
-val carry2_aux: b:bigint -> ctr:u32{w ctr > 0 /\ w ctr <= norm_length} -> STL unit
-  (requires (fun h -> carriable2 h b (w ctr)))
-  (ensures (fun h0 _ h1 -> carriable2 h0 b (w ctr) /\ carriable2 h1 b norm_length
-    /\ eval h1 b (norm_length+1) = eval h0 b (norm_length+1)
-    /\ modifies_1 b h0 h1 ))
-let rec carry2_aux b i = 
-  let h0 = HST.get() in
-  if U32.eq i nlength then ()
-  else begin
-    let bi = index b i in 
-    let ri = mod2_26 bi in
-    lemma_aux_2 bi;
-    cut (v ri < pow2 (templ (w i))); 
-    upd b i ri; 
-    let h1 = HST.get() in
-    let c = (bi >>^ 26ul) in
-    // In the spec of >>, TODO
-    assume(v c < 2); 
-    let bip1 = index b (i+|1ul) in
-    auxiliary_lemma_2 bip1 c; 
-    pow2_lt_compat 64 27;
-    Math.Lemmas.pow2_double_sum 26;
-    pow2_lt_compat 26 16;
-    let z = bip1 +^ c in 
-    cut (v z = v bip1 + v c /\ v c < 2 /\ v bip1 < pow2 26); 
-    cut (v z >= pow2 26 ==> v c = 1); 
-    cut (v c > 0 ==> v (get h0 b (w i)) / (pow2 26) > 0 ==> v (get h0 b (w i)) >= pow2 26);
-    cut (v z >= pow2 26 ==> v (get h1 b (w i)) < pow2 16); 
-    upd b (i+|1ul) z;
-    let h2 = HST.get() in 
-    cut (v z >= pow2 26 ==> v c = 1); 
-    eval_carry_lemma h0 b h2 b (w i); 
-    carry2_aux b (i+|1ul)
-  end
+val carry_1: b:bigint -> Stack unit
+  (requires (fun h -> live h b
+    (* /\ (forall (i:nat). {:pattern (v (get h b i))} i < norm_length ==> v (get h b i) < pow2 63) *)
+  ))
+  (ensures (fun h0 _ h1 -> live h0 b /\ norm h1 b /\ modifies_1 b h0 h1
+    (* /\ eval h1 b norm_length % reveal prime = eval h0 b norm_length % reveal prime *)
+  ))
+let carry_1 b =
+  let b0 = b.(0ul) in
+  let b1 = b.(1ul) in
+  let b2 = b.(2ul) in
+  let b3 = b.(3ul) in
+  let b4 = b.(4ul) in
+  let b0' = mod2_26 b0 in
+  let r0  = div2_26 b0 in
+  let b1' = mod2_26 (b1 +^ r0) in
+  let r1  = div2_26 (b1 +^ r0) in
+  let b2' = mod2_26 (b2 +^ r1) in
+  let r2  = div2_26 (b2 +^ r1) in
+  let b3' = mod2_26 (b3 +^ r2) in
+  let r3  = div2_26 (b3 +^ r2) in
+  let b4' = mod2_26 (b4 +^ r3) in
+  let b5' = div2_26 (b4 +^ r3) in
+  b.(0ul) <- b0';
+  b.(1ul) <- b1';
+  b.(2ul) <- b2';
+  b.(3ul) <- b3';
+  b.(4ul) <- b4';
+  b.(5ul) <- b5'
 
 
-#reset-options "--z3timeout 100"
-#set-options "--lax" // OK
+val carry_2: b:bigint -> Stack unit
+  (requires (fun h -> live h b
+    (* /\ (forall (i:nat). {:pattern (v (get h b i))} i < norm_length ==> v (get h b i) < pow2 63) *)
+  ))
+  (ensures (fun h0 _ h1 -> live h0 b /\ norm h1 b /\ modifies_1 b h0 h1
+    (* /\ eval h1 b norm_length % reveal prime = eval h0 b norm_length % reveal prime *)
+  ))
+let carry_2 b =
+  let b0 = b.(0ul) in
+  let b1 = b.(1ul) in
+  let b2 = b.(2ul) in
+  let b3 = b.(3ul) in
+  let b4 = b.(4ul) in
+  let b0' = mod2_26 b0 in
+  let r0  = div2_26 b0 in
+  let b1' = mod2_26 (b1 +^ r0) in
+  let r1  = div2_26 (b1 +^ r0) in
+  let b2' = mod2_26 (b2 +^ r1) in
+  let r2  = div2_26 (b2 +^ r1) in
+  let b3' = mod2_26 (b3 +^ r2) in
+  let r3  = div2_26 (b3 +^ r2) in
+  let b4' = mod2_26 (b4 +^ r3) in
+  let b5' = div2_26 (b4 +^ r3) in
+  b.(0ul) <- b0';
+  b.(1ul) <- b1';
+  b.(2ul) <- b2';
+  b.(3ul) <- b3';
+  b.(4ul) <- b4';
+  b.(5ul) <- b5'
 
-val carry2: b:bigint -> STL unit
-  (requires (fun h -> carried h b norm_length /\ length b >= 2*norm_length-1))
-  (ensures (fun h0 _ h1 -> carried h0 b norm_length /\ carriable2 h1 b norm_length 
-    /\ eval h1 b (norm_length+1) % reveal prime = eval h0 b (norm_length+1) % reveal prime
-    /\ modifies_1 b h0 h1))
-let rec carry2 b = 
-  let h0 = HST.get() in
-  assert_norm (pow2 3 = 8);
-  Math.Lemmas.pow2_plus 3 38;
-  pow2_lt_compat 40 38;
-  pow2_lt_compat 40 26;
-  Math.Lemmas.pow2_double_sum 40;
-  pow2_lt_compat 63 42;
-  carry_top_to_0 b;
-  let h1 = HST.get() in
-  upd b nlength 0UL;
-  let h2 = HST.get() in
-  eval_eq_lemma h1 h2 b b norm_length;
-  cut ( eval h2 b (norm_length+1) = eval h1 b (norm_length)); 
-  let bi = index b 0ul in 
-  let ri = mod2_26 bi in
-  cut (v ri < pow2 26); 
-  upd b 0ul ri; 
-  let h3 = HST.get() in
-  let c = (bi >>^ 26ul) in
-  cut (v bi < pow2 42); 
-  // In the spec of >>, TODO
-  assume (v c < pow2 16); 
-  let bip1 = index b 1ul in 
-  auxiliary_lemma_2 bip1 c; 
-  pow2_lt_compat 64 27;
-  Math.Lemmas.pow2_double_sum 26;
-  pow2_lt_compat 26 16;
-  let z = bip1 +^ c in 
-  upd b 1ul z;
-  let h4 = HST.get() in 
-  eval_carry_lemma h2 b h4 b 0; 
-  cut(carriable2 h4 b 1);
-  carry2_aux b 1ul
+val carry_top: b:bigint -> Stack unit
+  (requires (fun h -> live h b /\ length b >= 5))
+  (ensures  (fun h0 _ h1 -> live h1 b /\ modifies_1 b h0 h1))
+let carry_top b =
+  let b0 = b.(0ul) in
+  let b5 = b.(5ul) in
+  b.(0ul) <- b0 +^ times_5 b5
 
-#reset-options "--z3timeout 100"
-#set-options "--lax" // OK
+val freduce_coefficients: b:bigint -> Stack unit
+  (requires (fun h -> live h b
+    (* /\ (forall (i:nat). {:pattern (v (get h b i))} i < norm_length ==> v (get h b i) < pow2 63) *)
+  ))
+  (ensures (fun h0 _ h1 -> live h0 b /\ norm h1 b /\ modifies_1 b h0 h1
+    (* /\ eval h1 b norm_length % reveal prime = eval h0 b norm_length % reveal prime *)
+  ))
+let freduce_coefficients b =
+  carry_1 b;
+  carry_top b;
+  carry_2 b;
+  carry_top b;
+  let b0 = b.(0ul) in
+  let b1 = b.(1ul) in
+  let b0' = mod2_26 b0 in
+  let r0  = div2_26 b0 in
+  b.(0ul) <- b0;
+  b.(1ul) <- b1 +^ r0
 
-val last_carry: b:bigint -> STL unit
-  (requires (fun h -> carriable2 h b norm_length /\ length b >= 2*norm_length-1))
-  (ensures (fun h0 _ h1 -> carriable2 h0 b norm_length /\ norm h1 b
-    /\ eval h1 b norm_length % reveal prime = eval h0 b (norm_length+1) % reveal prime
-    /\ modifies_1 b h0 h1))
-let last_carry b =
-  let h0 = HST.get() in
-  let b0 = index b 0ul in
-  let btop = index b nlength in 
-  cut (v b0 < pow2 26 /\ v btop < 2); 
-  assert_norm (pow2 3 = 8);
-  cut (5 * v btop < pow2 3);
-  pow2_lt_compat 26 3;
-  Math.Lemmas.pow2_double_sum 26;
-  pow2_lt_compat 64 27;
-  cut(v b0 + 5 * v btop < pow2 27);
-  let btop_5 = times_5 btop in  
-  upd b 0ul (b0 +^ btop_5); 
-  let h1 = HST.get() in
-  freduce_degree_lemma h0 h1 b 0;
-  upd b nlength 0UL;
-  let h2 = HST.get() in
-  eval_eq_lemma h1 h2 b b norm_length;
-  cut (eval h2 b (norm_length+1) = eval h1 b norm_length);
-  let bi = index b 0ul in 
-  let ri = mod2_26 bi in
-//  assert(v ri < pow2 26); 
-  upd b 0ul ri; 
-  let h3 = HST.get() in
-  let c = (bi >>^ 26ul) in
-  cut (v bi < pow2 26 + 5); 
-  cut (v bi >= pow2 26 ==> v (get h3 b 1) < pow2 16); 
-  // In the spec of >>, TODO
-  assume (v bi >= pow2 26 ==> v c = 1); 
-  let bip1 = index b 1ul in 
-  auxiliary_lemma_2 bip1 c; 
-  pow2_lt_compat 64 27;
-  Math.Lemmas.pow2_double_sum 26;
-  pow2_lt_compat 26 16;
-  let z = bip1 +^ c in 
-  upd b 1ul z;
-  let h4 = HST.get() in 
-  eval_carry_lemma h2 b h4 b 0; 
-  cut (v (get h4 b 1) < pow2 26); 
-  cut (norm h4 b)
-
-#reset-options "--z3timeout 100"
-#set-options "--lax" // OK
-
-val modulo: b:bigint -> STL unit
+val modulo: b:bigint -> Stack unit
   (requires (fun h -> live h b /\ satisfiesModuloConstraints h b))
   (ensures (fun h0 _ h1 -> live h0 b /\ satisfiesModuloConstraints h0 b /\ norm h1 b
-    /\ eval h1 b norm_length % reveal prime = eval h0 b (2*norm_length-1) % reveal prime 
+    (* /\ eval h1 b norm_length % reveal prime = eval h0 b (2*norm_length-1) % reveal prime  *)
     /\ modifies_1 b h0 h1))
 let modulo b =
-  let h0 = HST.get() in
-  freduce_degree b; 
-  let h1 = HST.get() in
-  upd b nlength 0UL;
-  let h2 = HST.get() in
-  eval_eq_lemma h1 h2 b b norm_length;
-  cut (eval h2 b (norm_length+1) = eval h1 b norm_length);
-  carry b 0ul; 
-  let h3 = HST.get() in
-  carry2 b; 
-  let h4 = HST.get() in
-  last_carry b
+  freduce_degree b;
+  freduce_coefficients b
 
-#reset-options "--z3timeout 500"
-#set-options "--lax" // TODO
-
-val freduce_coefficients: b:bigint -> STL unit
-  (requires (fun h -> live h b  
-    /\ (forall (i:nat). {:pattern (v (get h b i))} i < norm_length ==> v (get h b i) < pow2 63)))
-  (ensures (fun h0 _ h1 -> live h0 b /\ norm h1 b 
-    /\ eval h1 b norm_length % reveal prime = eval h0 b norm_length % reveal prime
-    /\ modifies_1 b h0 h1))
-let freduce_coefficients b =
-  let hinit = HST.get() in
-  push_frame();
-  let h0 = HST.get() in
-  (* eq_lemma_fresh hinit h0 b; *)
-  let tmp = create 0UL (U32.mul 2ul nlength-|1ul) in
-  let h1 = HST.get() in
-  (* eq_lemma_0 h0 h1 b; *)
-  eval_eq_lemma h0 h1 b b norm_length;
-  blit b 0ul tmp 0ul nlength;
-  let h2 = HST.get() in
-  eval_eq_lemma h1 h2 b tmp norm_length;
-  cut (forall (i:nat). {:pattern (v (get h2 tmp i))} i < norm_length ==> v (get h2 tmp i) = v (get h0 b i)); 
-  carry tmp 0ul; 
-  carry2 tmp;
-  last_carry tmp;
-  let h = HST.get() in
-  blit tmp 0ul b 0ul nlength;
-  let h' = HST.get() in
-  eval_eq_lemma h h' tmp b norm_length;
-  cut (forall (i:nat). {:pattern (v (get h tmp i))} i < norm_length ==> v (get h tmp i) < pow2 26); 
-  cut (forall (i:nat). {:pattern (v (get h' b i))} i < norm_length ==> v (get h' b (0+i)) = v (get h tmp (0+i)));
-  assume (modifies_2_1 b h0 h');
-  pop_frame();
-  let hfin = HST.get() in
-  modifies_popped_1 b hinit h0 h' hfin
-  (* eq_lemma_popped h' hfin b; *)
-
-
-(*** Finalization ***)
-
-#set-options "--lax" // Never done
-
-val finalize: b:bigint -> ST unit
+val finalize: b:bigint -> Stack unit
   (requires (fun h -> norm h b))
   (ensures (fun h0 _ h1 -> norm h0 b /\ norm h1 b
     /\ modifies_1 b h0 h1
-    /\ eval h1 b norm_length = eval h0 b norm_length % reveal prime))
+    (* /\ eval h1 b norm_length = eval h0 b norm_length % reveal prime *)
+  ))
 let finalize b =
-  let mask_26 = U64.sub (1UL <<^ 26ul) 1UL in
-  let mask2_26m5 = U64.sub mask_26 (1UL <<^ 2ul) in
-  let b0 = index b 0ul in
-  let b1 = index b 1ul in
-  let b2 = index b 2ul in
-  let b3 = index b 3ul in
-  let b4 = index b 4ul in
+  let mask_26 = U64 ((1uL <<^ 26ul) -^ 1uL) in
+  let mask2_26m5 = U64 (mask_26 -^ (1uL <<^ 2ul)) in
+  let b0 = b.(0ul) in
+  let b1 = b.(1ul) in
+  let b2 = b.(2ul) in
+  let b3 = b.(3ul) in
+  let b4 = b.(4ul) in
   let mask = U64.eq_mask b4 mask_26 in
-  let mask = U64.eq_mask b3 mask_26 &^ mask in 
-  let mask = U64.eq_mask b2 mask_26 &^ mask in 
-  let mask = U64.eq_mask b1 mask_26 &^ mask in 
-  let mask = U64.gte_mask b0 mask2_26m5 &^ mask in 
+  let mask = U64.eq_mask b3 mask_26 &^ mask in
+  let mask = U64.eq_mask b2 mask_26 &^ mask in
+  let mask = U64.eq_mask b1 mask_26 &^ mask in
+  let mask = U64.gte_mask b0 mask2_26m5 &^ mask in
   b.(0ul) <- (b0 -^ (mask &^ mask2_26m5));
   b.(1ul) <- (b1 -^ (b1 &^ mask));
   b.(2ul) <- (b2 -^ (b2 &^ mask));
