examples/low-level/crypto/Crypto.Symmetric.Poly1305.fst
@@ -252,7 +252,7 @@ let add_and_multiply acc block r =
   cut (eval h1 acc 5 = eval h0 acc 5 + eval h0 block 5);
   bound27_isSum h0 h1 acc block;
   push_frame();
-  let tmp = create 0UL (U32.mul 2ul nlength-|1ul) in
+  let tmp = create 0UL (U32 (2ul *^ nlength -^ 1ul)) in
   let h2 = HST.get () in
   eval_eq_lemma h1 h2 acc acc norm_length;
   eval_eq_lemma h0 h2 r r norm_length;
@@ -669,12 +669,12 @@ let poly1305_update log msgB acc r =
 
 val append_as_seq_sub: h:mem -> n:UInt32.t -> m:UInt32.t -> msg:bytes{live h msg /\ w m <= w n /\ w n <= length msg} -> Lemma
   (append (as_seq h (Buffer.sub msg 0ul m))
- 	  (as_seq h (Buffer.sub (Buffer.offset msg m) 0ul (n -| m))) ==
+ 	  (as_seq h (Buffer.sub (Buffer.offset msg m) 0ul (U32 (n -^ m)))) ==
    as_seq h (Buffer.sub msg 0ul n))
 let append_as_seq_sub h n m msg =
   Seq.lemma_eq_intro
     (append (as_seq h (Buffer.sub msg 0ul m))
-   	    (as_seq h (Buffer.sub (Buffer.offset msg m) 0ul (n -| m))))
+   	    (as_seq h (Buffer.sub (Buffer.offset msg m) 0ul (U32 (n -^ m)))))
      (as_seq h (Buffer.sub msg 0ul n))
 
 (* Loop over Poly1305_update; could go below MAC *)
@@ -709,7 +709,7 @@ let rec poly1305_loop log msg acc r ctr =
       assert (ideal ==> sel_elem h1 acc == poly (ilog log1) (sel_elem h0 r));
       assert (ideal ==>
         ilog log1 == SeqProperties.snoc (ilog log) (encode_16 (sel_word h1 msg0)));
-      let log2 = poly1305_loop log1 msg1 acc r (ctr -| 1ul) in
+      let log2 = poly1305_loop log1 msg1 acc r (U32 (ctr -^ 1ul)) in
       let h2 = HST.get () in
       assert (norm h2 acc /\ modifies_1 acc h0 h2);
       lemma_modifies_1_trans acc h0 h1 h2;
@@ -722,7 +722,7 @@ let rec poly1305_loop log msg acc r ctr =
 	  //  (as_seq h0 (Buffer.sub msg1 0ul (UInt32.mul 16ul (ctr -| 1ul)))) ==
           //encode_pad (SeqProperties.snoc (ilog log) (encode_16 (sel_word h1 msg0)))
 	  //  (as_seq h0 (Buffer.sub (Buffer.offset msg 16ul) 0ul (UInt32.mul 16ul ctr -| 16ul))));
-	  encode_pad_snoc (ilog log) (as_seq h0 (Buffer.sub (Buffer.offset msg 16ul) 0ul (UInt32.mul 16ul ctr -| 16ul))) (sel_word h1 msg0);
+	  encode_pad_snoc (ilog log) (as_seq h0 (Buffer.sub (Buffer.offset msg 16ul) 0ul (U32 (16ul *^ ctr -^ 16ul)))) (sel_word h1 msg0);
 	  append_as_seq_sub h0 (UInt32.mul 16ul ctr) 16ul msg
 	  //assert (append (sel_word h1 msg0) (as_seq h0 (Buffer.sub (Buffer.offset msg 16ul) 0ul  (UInt32.mul 16ul ctr -| 16ul))) ==
           // (as_seq h0 (Buffer.sub msg 0ul (UInt32.mul 16ul ctr))))
